<?xml version="1.0" encoding="UTF-8"?>

<section xmlns:xi="http://www.w3.org/2001/XInclude">
  <title>Polynomial Functions</title>

  <introduction>
    <p>
      The simplest algebraic functions are constructed using the operations of addition and multiplication with a variable.
      While simple to construct, it is often difficult or even impossible to answer basic questions about these functions in general.
      However, these functions are extraordinarily important in nearly every branch of mathematics.
      We discuss foundational results about general polynomials in this section, and specialize to some easy to classify cases in the later sections.
    </p>
  </introduction>

  <definition>
    <title>Polynomial Function</title>
    <p>
      A <term>polynomial function</term>
      <idx>
	<h>Function</h>
	<h>Polynomial</h>
      </idx>
      of is a function of the form
      <me>f(x) = a_nx^n + a_{n-1}x^{n-1} + \cdots + a_1x + a_0,</me>
      where <m>n</m> is an integer, <m>a_0, a_1, \ldots, a_n</m> are numbers and <m>a_n \neq 0</m>.
    </p>
    <p>
      We say <m>f</m> is a polynomial of <term>degree</term>
      <idx>
	<h>Function</h>
	<h>Polynomial</h>
	<h>Degree</h>
      </idx>
      <m>n</m> and write <m>\deg{f} = n</m>.
      <usage>
	<notation>
	  <m>\deg{f}</m>
	</notation>
      </usage>
      The numbers <m>a_0, a_1, \ldots, a_n</m> are called the <term>coefficient</term>
      <idx>
	<h>Function</h>
	<h>Polynomial</h>
	<h>Coefficient</h>
      </idx>
      of <m>1, x, \ldots, x^n</m>, respectively.
    </p>
  </definition>
  
  <subsection>
    <title>Roots of Polynomials</title>

    <p>
      Polynomial functions are most interesting because they are relatively simple functions that allow us to model real world phenomena.
    </p>
    <example>
      <p>
	Assume an object is thrown straight up in the air.
	If we let <m>h_0</m> denote the distance from the thrower's hand to the ground when the object is released, and let <m>v_0</m> denote the velocity of the object in meters/second as it leaves the thrower's hand, then the height of the object as a function of time can be expressed using the polynomial
	<me>h(t) = -4.9t^2 + v_0t + h_0.</me>
      </p>
    </example>
    
    <question>
      <p>
	How long will it take for the object to return to the hand of the thrower?
      </p>
    </question>

    <p>
      To answer this question, we want the solutions to the equation
      <me>-4.9t^2 + v_0t + h_0 = h_0.</me>
      If we subtract <m>h_0</m> from both sides of the equation, then it is equivalent to find solutions to the polynomial equation
      <me>-4.9t^2 + v_0t = 0.</me>
      Questions of this type arise frequently when discussing polynomials.
    </p>
    
    <definition>
      <title>Root</title>
      A <term>root</term>
      <idx>
	<h>Function</h>
	<h>Polynomial</h>
	<h>Root</h>
      </idx>
      of the polynomial
      <me>f(x) = a_nx^n + a_{n-1}x^{n-1} + \cdots + a_1x + a_0</me>
      is a number, <m>r</m>, such that
      <me>0 = f(r) = a_nr^n + a_{n-1}r^{n-1} + \cdots + a_1 r + a_0.</me>
    </definition>

    <p>
      Questions about roots of polynomials have been posed and studied for millenia.
      One of the simplest questions asks whether we can find a formula that will produce the roots of a general polynomial of a certain degree in terms of its coefficients.
    </p>
    
    <question>
      <p>
	Is there a formula to find all of the roots of the polynomial <m>f(x) = a_nx^n + \cdots + a_0</m> in terms of the coefficients?
      </p>
    </question>

    <p>
      In general, the answer to this question is deeply unsatisfying.
      We will find formulas for polynomials of degree 1 in <xref ref="sec-linear_functions"/> and of degree 2 in <xref ref="sec-quadratic_functions"/>.
      While general formulas exist for polynomials of degree 3 and degree 4, they are beyond the scope of this text.
      However, there are no such general formulas for polynomials of degree 5 and higher.
      This means we will need to develop other techniques for finding roots of polynomials.
    </p>

    <theorem xml:id="thm-rational_root">
      <title>The Rational Root Theorem</title>
      <statement>
	<p>
	  Assume <m>p</m> and <m>q</m> are integers.
	  If <m>r = p/q</m> is a root of the polynomial
	  <me>f(x) = a_nx^n + a_{n-1}x^{n-1} + \cdots + a_1x + a_0,</me>
	  then <m>p</m> is a divisor of <m>a_0</m> and <m>q</m> is a divisor of <m>a_n</m>.
	</p>
      </statement>
    </theorem>

    <example xml:id="example-rational_root">
      <p>
	Find all rational roots of <m>f(x) = 2x^4 - 7x^3 + 5x^2 - 7x + 3</m>.
      </p>
      <solution>
	<p>
	  The divisors of <m>2</m> are <m>\pm 2</m> and <m>\pm 1</m>.
	  The divisors of <m>3</m> are <m>\pm 1</m>, <m>\pm 3</m>.
	  <xref ref="thm-rational_root" text="title"/> tells us the only possible rational numbers that can be roots of <m>f</m> are
	  <me>\pm 3,\, \pm \frac{3}{2},\, \pm 1,\,\text{and}\ \pm\frac{1}{2}.</me>
	  We can check each of these by evaluating the function at these rational numbers.
	  <md>
	    <mrow> f(3) \amp= 2(3)^4 - 7(3)^3 + 5(3)^2 - 7(3) + 3 = 0 </mrow>
	    <mrow>f(-3) \amp= 2(-3)^4 - 7(-3)^3 + 5(-3)^2 - 7(-3) + 3 = 420</mrow>
	    <mrow>f\left(\frac{3}{2}\right) \amp= 2\left(\frac{3}{2}\right)^4 - 7\left(\frac{3}{2}\right)^3 + 5\left(\frac{3}{2}\right)^2 - 7\left(\frac{3}{2}\right) + 3 = -\frac{39}{4}</mrow>
	    <mrow>f\left(-\frac{3}{2}\right) \amp= 2\left(-\frac{3}{2}\right)^4 - 7\left(-\frac{3}{2}\right)^3 + 5\left(-\frac{3}{2}\right)^2 - 7\left(-\frac{3}{2}\right) + 3  = \frac{117}{2}</mrow>
	    <mrow>f(1) \amp= 2(1)^4 - 7(1)^3 + 5(1)^2 - 7(1) + 3 = -4</mrow>
	    <mrow>f(-1)\amp = 2(-1)^4 - 7(-1)^3 + 5(-1)^2 - 7(-1) + 3 = 24</mrow>
	    <mrow>f\left(\frac{1}{2}\right) \amp= 2\left(\frac{1}{2}\right)^4 - 7\left(\frac{1}{2}\right)^3 + 5\left(\frac{1}{2}\right)^2 - 7\left(\frac{1}{2}\right) + 3 = 0</mrow>
	    <mrow>f\left(-\frac{1}{2}\right)\amp = 2\left(-\frac{1}{2}\right)^4 - 7\left(-\frac{1}{2}\right)^3 + 5\left(-\frac{1}{2}\right)^2 - 7\left(-\frac{1}{2}\right) + 3 = \frac{35}{4}.</mrow>
	  </md>
	  Therefore the only rational roots of the polynomial <m>f</m> are <m>x = 3</m> and <m>x = 1/2</m>.
	</p>
      </solution>
    </example>
  </subsection>
  
  <subsection>
    <title>Polynomial Division</title>
    <p>
      Another method for finding roots that is often paired with <xref ref="thm-rational_root" text="title"/> is division.
      Recall that if we have an integer <m>n</m> and a smaller integer, <m>d</m>, then we can always find integers <m>q</m> and <m>r</m> with <m>r \lt d</m> such that
      <me>n = qd + r.</me>
      There is an analogous result for polynomials.
    </p>
    
    <theorem xml:id="thm-polynomial_division">
      <title>Polynomial Division</title>
      <statement>
	<p>
	  Assume <m>f</m> and <m>d</m> are polynomials with <m>\deg{d} \lt \deg{f}</m>.
	  There exist polynomials <m>q</m> and <m>r</m> with <m>\deg{r} \lt \deg{d}</m> such that
	  <me>f(x) = q(x)d(x) + r(x)</me>.
	</p>
	<p>
	  In analogy with the integers, we call the polynomials <m>d</m> the <term>dividend</term>, <m>q</m> the <term>quotient</term>, and <m>r</m> the <term>remainder</term>, and 
	  we say that <m>f</m> divided by <m>d</m> is <m>q</m> with remainder <m>r</m>
	</p>
      </statement>
    </theorem>

    <definition>
      <p>
	Assume <m>f</m> and <m>d</m> are polynomials.
	The polynomial <m>g</m> <term>divides</term>
	<idx>
	  <h>Function</h>
	  <h>Polynomial</h>
	  <h>Divides</h>
	</idx>
	the polynomial <m>f</m> if the remainder in <xref ref="thm-polynomial_division"/> satisfies <m>r(x) = 0</m>.
      </p>
    </definition>

    <p>
      For integers <m>n</m> and <m>d</m>, the process of finding <m>q</m> and <m>r</m> is often performed using long division.
    </p>

    <example xml:id="example-integer_division">
      <p>
	To divide <m>6935</m> by <m>30</m>, we would perform the long division using the symbols
	<md>
	  <mrow>\amp\phantom{)}231</mrow>
	  <mrow>30 \amp\overline{\smash{)}{6935}} </mrow>
	  <mrow>\amp \underline{-60}</mrow>
	  <mrow>\amp \phantom{lllll}93</mrow>
	  <mrow>\amp \phantom{lll}\underline{-90}</mrow>
	  <mrow>\amp \phantom{lllllll}35</mrow>
	  <mrow>\amp \phantom{llll}\underline{-30}</mrow>
	  <mrow>\amp \phantom{lllllllll}5</mrow>
	</md>
	to find <m>6935 = 30 \times 231 + 5</m>.
      </p>
    </example>
    
    <p>
      To understand how to perform division with polynomials, it is helpful to understand how the division algorithm with numbers written in base <m>10</m>.
      The four steps in the long division above are shorthand for the following equations.
    </p>
    <mdn>
      <mrow xml:id="eq-division_1">6935 \amp= 30 \times 200 + 935</mrow>
      <mrow xml:id="eq-division_2">935 \amp= 30 \times 30 + 35</mrow>
      <mrow xml:id="eq-division_3">35 \amp= 30 \times 1 + 5</mrow>
    </mdn>
    <p>
      We arrive at the final answer by repeated substitution for the remainders starting with <xref ref="eq-division_1"/>.
    </p>
    <md>
      <mrow>
	6935 \amp= 30 \times 200 + 935 \amp\amp \text{Substitute the RHS of}\ <xref ref="eq-division_2"/>\ \text{for}\ 935
      </mrow>
      <mrow>
	\amp = 30 \times 200 + 30 \times 30 + 35 \amp\amp \text{Substitue the RHS of}\ <xref ref="eq-division_3"/>\ \text{for}\ 35
      </mrow>
      <!-- <mrow> -->
      <!-- 	\amp = 30 \times 200 + 30 \times 30 + 30 \times 1 + 5 \amp\amp \text{Substitute the RHS of}\ <xref ref="eq-division_4"/>\ \text{for}\ 5 -->
      <!-- </mrow> -->
      <mrow>
	\amp = 30 \times 200 + 30 \times 30 + 30 \times 1 + 5 \amp\amp \text{Factor}\ 3\ \text{from the first three terms}
      </mrow>
      <mrow>
	\amp= (200 + 30 + 1) \times 3 + 2 \amp\amp \text{Simplify}
      </mrow>
      <mrow>
	\amp = 231 \times 30 + 5.
      </mrow>
    </md>
    <p>
      This process terminates because at each stage we are reducing the number of digits in the remainder by at least one.
      When we do long division with polynomials, our goal will be similar, but we will reduce the degree of the remainder polynomial by at least one.
    </p>

    <example>
      <p>
	To divide the polynomial <m>f(x) = 6x^3 + 9x^2 + 3x + 5</m> by the polynomial <m>d(x) = 3x</m>, we write
	<mdn>
	  <mrow xml:id="eq-poly_div_1">6x^3 + 9x^2 + 3x + 5 \amp= 2x^2 \times 3x + 9x^2 + 3x + 5</mrow>
	  <mrow xml:id="eq-poly_div_2">9x^2 + 3x + 5 \amp= 3x \times 3x + 3x + 5</mrow>
	  <mrow xml:id="eq-poly_div_3">3x + 5 \amp= 1 \times 3x + 5</mrow>
	</mdn>
	then, starting from <xref ref="eq-poly_div_1"/>, we substitute for the remainders
	<md>
	  <mrow>6x^3 + 9x^2 + 3x + 5 \amp = 2x^2 \times 3x + 9x^2 + 3x + 5 \amp\amp \text{Substitute using}\ <xref ref="eq-poly_div_2"/></mrow>
	  <mrow>\amp= 2x^2 \times 3x + 3x \times 3x + 3x + 5 \amp\amp \text{Substitute using}<xref ref="eq-poly_div_3"/></mrow>
	  <mrow>\amp= 2x^2 \times 3x + 3x \times 3x + 1 \times 3x + 5 \amp\amp \text{Factor}</mrow>
	  <mrow>\amp= (2x^2 + 3x + 1) \times 3x + 5.</mrow>
	</md>
	Therefore <m>f(x) = 6x^3 + 9x^2 + 3x + 5</m> divided by <m>d(x) = 3x</m> is <m>q(x) = 2x^2 + 3x + 1</m> with remainder <m>r(x) = 5</m>.
      </p>
      <p>
	We can also perform polynomial division using the same shorthand as we would for numbers.
	When performing polynomial division in this way, it is important to carefully distribute signs when subtracting.
      </p>
      <md>
	<mrow>\amp\phantom{)}2x^2 + 3x + 1</mrow>
	<mrow>3x \amp\overline{\smash{)}{6x^3 + 9x^2 + 3x + 5}} </mrow>
	<mrow>\amp \underline{-6x^3}</mrow>
	<mrow>\amp \phantom{lllll}0 + 9x^2</mrow>
	<mrow>\amp \phantom{lllllllll}\underline{-9x^2}</mrow>
	<mrow>\amp \phantom{6x^3 + 9x^2}0 + 3x</mrow>
	<mrow>\amp \phantom{6x^3 + 9x^2 0l}\underline{- 3x}</mrow>
	<mrow>\amp \phantom{6x^3 + 9x^2 + 3}0 + 5</mrow>
      </md>
    </example>

    <remark>
      <p>
	Note that if we evaluate each of the polynomials at <m>x = 10</m>, then we find
	<me>f(10) = 6000 + 900 + 30 + 5 = 6935</me>
	divided by <m>d(10) = 30</m> is
	<me>q(10) = 200 + 30 + 1 = 231</me>
	with remainder <m>r(10) = 5</m>.
	Indeed, polynomial long division is a generalization of long division in base <m>10</m>.
      </p>
    </remark>

    <p>
      When paired with <xref ref="thm-rational_root" text="title"/>, polynomial long division is useful for factoring polynomials.
      The main tool is the following theorem.
    </p>
    
    <theorem xml:id="thm-root_div">
      <statement>
	<p>
	  The number <m>r</m> is a root of the polynomial <m>f</m> if and only if <m>(x - r)</m> divides <m>f</m>.
	</p>
      </statement>
    </theorem>

    <definition>
      <p>
	Assume <m>f</m> is a polynomial and <m>r</m> is a root of <m>f</m>.
	The <term>multiplicity</term> of <m>r</m> is the largest integer <m>m</m> such that <m>(x - r)^m</m> divides <m>f</m>
      </p>
    </definition>

    <example>
      <p>
	As we saw in <xref ref="example-rational_root"/>, the polynomial <m>f(x) = 2x^4 - 7x^3 + 5x^2 - 7x + 3</m> has a root at <m>x = 1/2</m> and at <m>x = 3</m>.
	By <xref ref="thm-root_div"/>, the polynomial <m>x - 1/2</m> divides <m>f(x)</m>
      </p>
      <md>
	<mrow>\amp\phantom{)}2x^3 - 6x^2 + 2x - 6</mrow>
	<mrow>x - \frac{1}{2} \amp\overline{\smash{)}{2x^4 - 7x^3 + 5x^2 - 7x + 3}} </mrow>
	<mrow>\amp \underline{-2x^4 + x^3}</mrow>
	<mrow>\amp \phantom{)2x^4}-6x^3 + 5x^2</mrow>
	<mrow>\amp \phantom{)2x^4}\underline{+6x^3 - 3x^2}</mrow>
	<mrow>\amp \phantom{)2x^4 - 7x^3 +}2x^2 - 7x</mrow>
	<mrow>\amp \phantom{)2x^4 - 7x^3}\underline{-2x^2 + 2x}</mrow>
	<mrow>\amp \phantom{)2x^4 - 7x^3 + 5x^2}-6x + 3</mrow>
	<mrow>\amp \phantom{)2x^4 - 7x^3 + 5x^2}\underline{+6x - 3}</mrow>
	<mrow>\amp \phantom{)2x^4 - 7x^3 + 5x^2 - 7x +}0</mrow>
      </md>
      <p>
	This allows us to write
	<me>f(x) = \left(x - \frac{1}{2}\right)\left(2x^3 - 6x^2 + 2x - 6\right).</me>
      </p>
      <p>
	Since <m>f(3) = 0</m> and <m>3 - 1/2 \neq 0</m>, we conclude that <m>x - 3</m> divides <m>2x^3 - 6x^2 + 2x - 6</m>.
      </p>
      <md>
	<mrow>\amp\phantom{)}2x^2 + 2</mrow>
	<mrow>x - 3 \amp\overline{\smash{)}{2x^3 - 6x^2 + 2x - 6}} </mrow>
	<mrow>\amp \underline{-2x^3 + 6x^2}</mrow>
	<mrow>\amp \phantom{)2x^3}0 + 2x - 6</mrow>
	<mrow>\amp \phantom{)2x^3-}\underline{-2x + 6}</mrow>
	<mrow>\amp \phantom{)2x^3 - 6x^2 + }0</mrow>
      </md>
      <p>
	Hence we have the factorization
      </p>
      <md>
	<mrow>f(x) \amp= \left(x - \frac{1}{2}\right)(x - 3)(2x^2 + 2)</mrow>
	<mrow>\amp = \left(x - \frac{1}{2}\right)(x - 3)(2)(x^2 + 1)</mrow>
	<mrow>\amp = 2\left(x - \frac{1}{2}\right)(x - 3)(x^2 + 1)</mrow>
	<mrow>\amp = (2x - 1)(x - 3)(x^2 + 1).</mrow>
      </md>
    </example>
  </subsection>
  
  <theorem xml:id="thm-fundamental_theorem">
    <title>The Fundamental Theorem of Algbera</title>
    <creator>Carl Friedrich Gauss</creator>
    <statement>
      <p>
	Every polynomial of degree <m>n > 0</m> has at least one root, which may be a complex number of the form
	<m>a + bi = a + b\sqrt{-1}</m>.
      </p>
    </statement>
  </theorem>

</section>
