<?xml version="1.0" encoding="UTF-8"?>

<section xml:id="sec-quadratic_functions" xmlns:xi="http://www.w3.org/2001/XInclude">
  <title>Forms of Quadratic Functions</title>
  <objectives>
    <ul>
      <li>
	find the vertex of a quadratic function,
      </li>
      <li>
	find the <m>x</m>-intercept(s) of a quadratic function
      </li>
      <li>
	find the <m>y</m>-intercept of a quadratic functions,
      </li>
      <li>
	find the line of symmetry of a quadratic functions, and
      </li>
      <li>
	graph a quadratic function.
      </li>
    </ul>
  </objectives>

  <introduction>
    <p>
      In this section, we study a polynomial functions of degree 2.
      These polynomial functions are often called <em>quadratic function</em>.
    </p>
  </introduction>

  <definition xml:id="def-quadratic_function">
    <title>Quadratic Function</title>
    <p>
      A function <m>f \colon \R \to \R</m> is <term>quadratic</term>
      <idx>
	<h>Function</h>
	<h>Quadratic</h>
      </idx>
      if it has the form
      <me>f(x) = ax^2 + bx + c
      \quad\text{or}\quad
      y = ax^2 + bx + c,</me>
      where <m>a</m>, <m>b</m>, and <m>c</m> are numbers, and <m>a \neq 0</m>.
    </p>
  </definition>

  <subsection>
    <title>Vertex Form</title>
    <p>
      Just as with lines, quadratic functions are easier to understand through visualizations.
      While general quadratics are slightly more complicated, we can already handle quadratics in the following form.
    </p>

    <definition>
      <title>The Vertex Form of a Quadratic</title>
      <p>
	A quadratic function, <m>f(x)</m>, is in <term>vertex form</term>
	<idx>
	  <h>Function</h>
	  <h>Quadratic</h>
	  <h>Vertex Form</h>
	</idx>
	if there are numbers <m>h</m> and <m>k</m> such that
	<me>f(x) = a(x - h)^2 + k.</me>
      </p>
    </definition>
    
    <p>
      The methods of <xref ref="sec-transformations"/> tell us how to graph a quadratic in vertex form using <xref ref="fig-parabola" text="title"/>.
      We call the graph of <m>y = x^2</m> a <term>parabola</term>
      <idx>
	<h>Graph</h>
	<h>Parabola</h>
      </idx>
      and the point <m>(0,0)</m> the <term>vertex</term> 
	<idx>
	  <h>Graph</h>
	  <h>Parabola</h>
	  <h>Vertex</h>
	</idx>
	of the parabola.
    </p>
    
    <p>
      To graph of the quadratic function <m>y = a(x - h)^2 + k</m>
      <ol>
	<li>
	  <p>
	    Translate the graph of <m>y = x^2</m> horizontally by <m>h</m> units.
	    <ul>
	      <li>If <m>0 \lt h</m>, then the translation is to the right.</li>
	      <li>If <m>h \lt 0</m>, then the translation is to the left.</li>
	    </ul>
	    This operation translates the vertex from <m>(0,0)</m> to <m>(h,0)</m>.
	  </p>
	</li>
	<li>
	  <p>
	    Scale the graph of <m>(x - h)^2</m> by <m>\abs{a}</m>.
	    <ul>
	      <li>If <m>1 \lt a</m>, then the graph is stretched.</li>
	      <li>If <m>a \lt 1</m>, then the graph is compressed.</li>
	    </ul>
	    This operation fixes the vertex at <m>(h,0)</m>.
	  </p>
	</li>
	<li>
	  <p>
	    If <m>a \lt 1</m>, reflect the graph of <m>\abs{a}(x - h)^2</m> over the <m>x</m>-axis
	    This operation fixes the vertex at <m>(h,0)</m>.
	  </p>.
	</li>
	<li>
	  <p>
	    Translate the graph of <m>a(x - h)^2</m> vertically by <m>k</m> units.
	    <ul>
	      <li>If <m>k \lt 0</m>, then the translation is down.</li>
	      <li>If <m>0 \lt k</m>, then the translation is up.</li>
	    </ul>
	    This operation translates the vertex to <m>(h,k)</m>.
	  </p>
	</li>
      </ol>
      This tells us a quadratic function in the form
      <me>y = a(x - h)^2 + k</me>
      is a parabola with vertex at <m>(h,k)</m>.
    </p>
  </subsection>
  
  <subsection xml:id="subsec-completing_the_square">
      <title>Completing the Square</title>
      <introduction>
	<p>
	  Surprisingly, every quadratic function can be placed into vertex form.
	  Paired with the observations above, this tells us the graph of <em>every</em> quadratic function is a parabola.
	  Placing a general quadratic function into vertex form will require the method of completing the square.
	</p>
      </introduction>
      
      <p>
	Remember that when we multiply two binomials, we must distribute.
	We can remember how to distribute using the mnemonic FOIL: <alert>F</alert>irst, <alert>O</alert>uter, <alert>I</alert>nner, <alert>L</alert>ast:
      </p>
      <figure>
	<caption> Multiplying binomials using the FOIL method.</caption>
	<image source="images/FOIL.png"/>
      </figure>
      <p>
	If we use this method to multiply a binomial by itself, then we find the useful formula
	<md>
	  <mrow>
	    (x + h)^2 \amp = (x + h)(x + h)
	  </mrow>
	  <mrow>\amp = xx + xh + hx + hh</mrow>
	  <mrow>\amp = x^2 + hx + hx + h^2</mrow>
	  <mrow>\amp = x^2 + 2hx + h^2.</mrow>
	</md>
	We call a quadratic function of the form <m>y = x^2 + 2hx + h^2</m> a <term>perfect square</term>.
	<idx>
	  <h>Perfect Square</h>
	</idx>
      </p>

      <p>
	Given a quadratic equation <m>f(x) = ax^2 + bx + c</m>, we can use the formula
	<me>(x + h)^2 = x^2 + 2hx + h^2 </me>
	to <term>complete the square</term>
	<idx>
	  <h>Complete the Square</h>
	</idx>
	as follows.
      </p>
      <algorithm xml:id="alg-completing_the_square">
	<title>Completing the Square</title>
	<p>
	  To complete the square with the quadratic function <m>f(x) = ax^2 + bx + c</m>
	</p>
	<ol>
	  <li>
	    Factor an <m>a</m> from the first two terms to get
	    <me>f(x) = a\left(x^2 + \frac{b}{a}x\right) + c.</me>
	  </li>
	  <li>
	    Add and subtract <m>\left(\frac{b}{2a}\right)^2</m> inside the parentheses to get
	    <me>
	      f(x) = a\left(x^2 + \frac{b}{a}x + \left(\frac{b}{2a}\right)^2 - \left(\frac{b}{2a}\right)^2 \right) + c
	    </me>
	  </li>
	  <li>
	    Factor the first three terms inside the parentheses as a perfect square
	    <me>f(x) = a\left(\left(x + \frac{b}{2a}\right)^2 - \left(\frac{b}{2a}\right)^2 \right) + c</me>
	  </li>
	  <li>
	    Distribute the <m>a</m> through the sum
	    <me>f(x) = a\left(x + \frac{b}{2a}\right)^2 - a\left(\frac{b}{2a}\right)^2 + c.</me>
	  </li>
	</ol>
      </algorithm>

      <p>
	The result of completing the square is almost the vertex form for the quadratic function.
	We just need to rewrite the term
	<me>x + \frac{b}{2a} = x - \left(-\frac{b}{2a}\right)</me>
	so that 
	<me>f(x) = a\left(x - \left(-\frac{b}{2a}\right)\right)^2 - a\left(\frac{b}{2a}\right)^2 + c.</me>
	The number
	<m>h = -\frac{b}{2a}</m>
	is the <m>x</m>-coordinate of the vertex, and the number
	<md>
	  <mrow>k \amp= - a\left(\frac{b}{2a}\right)^2 + c</mrow>
	  <mrow>\amp= -a\left(\frac{b^2}{4a^2}\right) + c</mrow>
	  <mrow>\amp= -\frac{b^2}{4a} + \frac{4ac}{4a}</mrow>
	  <mrow>\amp = - \frac{b^2 - 4ac}{4a}.</mrow>
	</md>
	is the <m>y</m>-coordinate of the vertex.
      </p>
      
      <example>
	<statement>
	  <p>
	    Find the vertex of the quadratic function <m>f(x) = x^2 + 4x + 5</m>.
	  </p>
	</statement>
	<solution>
	  <p>
	    When the coefficient on <m>x^2</m> is 1, we can skip the first step and the last step:
	  </p>
	  <md>
	    <mrow>f(x) \amp = x^2 + 4x + 5 \amp\amp \text{Add and subtract}\ \left(\frac{4}{2}\right)^2 = 2^2</mrow>
	    <mrow>\amp= x^2 + 4x + 2^2 - 2^2 + 5 \amp\amp \text{Factor}</mrow>
	    <mrow>\amp = (x + 2)^2 - 2^2 + 5 \amp\amp \text{Simplify}</mrow>
	    <mrow>\amp = (x + 2)^2 - 4 + 5 \amp\amp \text{Simplify}</mrow>
	    <mrow>\amp = (x + 2)^2 + 1.</mrow>
	  </md>
	  <p>
	    The vertex of the quadratic function <m>f(x) = x^2 + 4x + 5</m> is <m>(-2, 1)</m>.
	  </p>
	</solution>
      </example>
      <example>
	<statement>
	  <p>
	    Find the vertex of the quadratic function <m>f(x) = 3x^2 - 4x + 5</m>.
	  </p>
	</statement>
	<solution>
	  <p>
	    When the coefficient on <m>x</m> is a negative number, we can still use the formula by rewriting the subtraction as addition with a negative number.
	  </p>
	  <md>
	    <mrow>f(x) \amp = 3x^2 - 4x + 5 \amp\amp \text{Rewrite}</mrow>
	    <mrow>\amp = 3x^2 + (-4)x + 5 \amp\amp \text{Factor}\ 3\ \text{from the first two terms}</mrow>
	    <mrow>\amp= 3\left(x^2 + \left(-\frac{4}{3}\right)x\right) + 5 \amp\amp \text{Add and subtract}\ \left(\frac{\frac{4}{3}}{2}\right)^2 = \left(\frac{2}{3}\right)^2</mrow>
	    <mrow>\amp = 3\left(x^2 + \left(-\frac{4}{3}\right)x +  \left(-\frac{2}{3}\right)^2 - \left(-\frac{2}{3}\right)^2\right) + 5\amp\amp \text{Factor}</mrow>
	    <mrow>\amp = 3\left(\left(x + \left(-\frac{2}{3}\right)\right)^2 - \frac{4}{9}\right) + 5 \amp\amp \text{Distribute}</mrow>
	    <mrow>\amp = 3\left(x - \frac{2}{3}\right)^2 - \frac{4}{3} + \frac{15}{3} \amp\amp \text{Simplify}</mrow>
	    <mrow>\amp = 3\left(x - \frac{2}{3}\right)^2 + \frac{11}{3}.</mrow>
	  </md>
	  <p>
	    The vertex of the quadratic function <m>f(x) = 3x^2 -4x + 5</m> is <m>\left(\frac{2}{3}, \frac{11}{3}\right).</m>
	  </p>
	</solution>
      </example>

      <p>
	Given a quadratic function
	<m>f(x) = ax^2 + bx + c</m>,
	we will often want to find the vertex of the parabola without having to complete the square.
	We can use our observations above.
      </p>
      <claim xml:id="vertex_formula">
	<title>The Vertex Formula</title>
	<statement>
	  <p>
	    Let <m>f(x) = ax^2 + bx + c</m> be a quadratic function.
	    The <m>x</m>-coordinate of the vertex is
	    <me>h = -\frac{b}{2a}</me>
	    and the <m>y</m>-coordinate of the vertex is
	    <me>k = f(h) = f\left(-\frac{b}{2a}\right).</me>
	  </p>
	</statement>
      </claim>

      <p>
	This formula allows us to place the quadratic function <m>f(x) = ax^2 + bx + c</m> into vertex form very easily:
	<me>f(x) = a\left(x + \frac{b}{2a}\right) + k.</me>
      </p>
      
      <example>
	<statement>
	  <p>
	    Use the <xref ref="vertex_formula" text="title"/> to place the quadratic function <m>f(x) = 3x^2 + 2x + 7</m> into vertex form.
	  </p>
	</statement>
	<solution>
	  <p>
	    By <xref ref="vertex_formula" text="title"/>, the <m>x</m>-coordinate of the vertex is
	    <me>h = -\frac{2}{2(3)} = -\frac{1}{3}.</me>
	    The <m>y</m>-coordinate of the vertex is
	    <md>
	      <mrow>k \amp= f\left(-\frac{1}{3}\right) </mrow>
	      <mrow>\amp= 3\left(-\frac{1}{3}\right)^2 + 2\left(-\frac{1}{3}\right) + 7</mrow>
	      <mrow>\amp= 3\left(\frac{1}{9}\right) - \frac{2}{3} + 7</mrow>
	      <mrow>\amp= \frac{1}{3} - \frac{2}{3} + \frac{3}{3}7</mrow>
	      <mrow>\amp = \frac{1 - 2 + 21}{3}</mrow>
	      <mrow>\amp = \frac{20}{3}</mrow>
	    </md>
	  </p>
	  <p>
	    We can check our answer by simply expanding the vertex form
	    <md>
	      <mrow>3\left(x - \left(-\frac{1}{3}\right)\right)^2 + \frac{20}{3} \amp= 3\left(x + \frac{1}{3}\right)^2 + \frac{20}{3}</mrow>
	      <mrow>\amp= 3\left(x^2 + \frac{2}{3}x + \frac{1}{9}\right) + \frac{20}{3}</mrow>
	      <mrow>\amp= 3x^2 + 2x + \frac{1}{3} + \frac{20}{3}</mrow>
	      <mrow>\amp= 3x^2 + 2x + \frac{21}{3}</mrow>
	      <mrow>\amp = 3x^2 + 2x + 7 = f(x).</mrow>
	    </md>
	  </p>
	</solution>
      </example>
    </subsection>
</section>
