<?xml version="1.0" encoding="UTF-8"?>

<section xml:id="sec-transformations" xmlns:xi="http://www.w3.org/2001/XInclude">
  <title>Graph Transformations</title>

  <introduction>
    <p>
      Graphing arbitrary functions can be a difficult task and the general methods are beyond the scope of basic algebra.
      However, if we know the graph of a function, <m>f</m>, and we can write another function, <m>g</m>, in terms of <m>f</m> in a specific way, then we can use the graph of <m>f(x)</m> to graph <m>g(x)</m> using <em>transformations</em>.
      In this seciton, we discuss three types of transformations: translation, scaling, and reflection.
    </p>
  </introduction>

  <subsection>
    <title>Translation</title>
    <introduction>
      <p>
	Throughout this section, assume that the graph of the function <m>y = f(x)</m> is known.
      </p>
    </introduction>
    
    <subsubsection>
      <title>Vertical Translation</title>
      
      <definition xml:id="def-vertical_translation">
	<title>Vertical Translation</title>
	<p>
	  Let <m>c</m> be a positive number.
	  We say the function <m>g(x)</m> is a <term>vertical translation</term>
	  <idx>
	    <h>Graph</h>
	    <h>Tranformation</h>
	    <h>Translation</h>
	    <h>Vertical</h>
	  </idx>
	  of the function <m>f(x)</m> if <m>g(x) = f(x) \pm c</m>.
	</p>
	<ul>
	  <li>
	    <p>
	      The graph of <m>g(x) = f(x) + c</m> is obtained by shifting the graph of <m>y = f(x)</m> up the <m>y</m>-axis by <m>c</m> units.
	    </p>
	  </li>
	  <li>
	    <p>
	      The graph of <m>g(x) = f(x) - c</m> is obtained by shifting the graph of <m>y = f(x)</m> down the <m>y</m>-axis by <m>c</m>-units.
	    </p>
	  </li>
	</ul>
      </definition>
      
      <example>
	<statement>
	  <p>
	    Use <xref ref="fig-parabola" text="title"/> to graph the functions <m>g(x) = x^2 + 2</m> and <m>h(x) = x^2 - 3</m>.
	  </p>
	</statement>
	<solution>
	  <p>
	    The graph of <m>g(x)</m> is obtained by shifting the graph of <m>f(x)</m> up the <m>y</m>-axis by <m>2</m> units, and the graph of <m>h(x)</m> is obtained by shifting the graph of <m>f(x)</m> down the <m>y</m>-axis by 3 units.
	  </p>
	  <figure>
	    <image>
	      <latex-image>
		<xi:include parse="text" href="tex/transformations/vertical_translation.tex"/>
	      </latex-image>
	    </image>
	  </figure>
	</solution>
      </example>
    </subsubsection>
    
    <subsubsection>
      <title>Horizontal Translation</title>

      <definition xml:id="def-horizontal_translation">
	<title>Horizontal Translation</title>
	<p>
	  Let <m>c</m> be a positive number.
	  We say the function <m>g(x)</m> is a <term>horizontal translation</term>
	  <idx>
	    <h>Graph</h>
	    <h>Tranformation</h>
	    <h>Translation</h>
	    <h>Horizontal</h>
	  </idx>
	  of the function <m>f(x)</m> if <m>g(x) = f(x \pm c)</m>.
	</p>
	<ul>
	  <li>
	    <p>
	      The graph of <m>g(x) = f(x - c)</m> is obtained by shifting the graph of <m>y = f(x)</m> to the right along the <m>x</m>-axis by <m>c</m> units.
	    </p>
	  </li>
	  <li>
	    <p>
	      The graph of <m>g(x) = f(x + c)</m> is obtained by shifting the graph of <m>y = f(x)</m> to the left along the <m>x</m>-axis by <m>c</m>-units.
	    </p>
	  </li>
	</ul>
      </definition>

      <example>
	<statement>
	  <p>
	    Use <xref ref="fig-parabola" text="title"/> to graph the functions <m>g(x) = (x+2)^2</m> and <m>h(x) = (x-3)^2</m>.
	  </p>
	</statement>
	<solution>
	  <p>
	    The graph of <m>g(x)</m> is obtained by shifting the graph of <m>f(x)</m> to the left along the <m>x</m>-axis by <m>2</m> units, and the graph of <m>h(x)</m> is obtained by shifting the graph of <m>f(x)</m> to the right along the <m>x</m>-axis by 3 units.
	  </p>
	  <figure>
	    <image>
	      <latex-image>
		<xi:include parse="text" href="tex/transformations/horizontal_translation.tex"/>
	      </latex-image>
	    </image>
	  </figure>
	</solution>
      </example>
    </subsubsection>

  </subsection>

  

  <subsection>
    <title>Scaling</title>

    <subsubsection>
      <title>Vertical Scaling</title>

      <definition xml:id="def-vertical_scaling">
	<title>Vertical Scaling</title>
	<p>
	  Let <m>c > 1</m> be a number.
	  We say the function <m>g(x)</m> is a <term>vertical scaling</term>
	  <idx>
	    <h>Graph</h>
	    <h>Tranformation</h>
	    <h>Scaling</h>
	    <h>Vertical</h>
	  </idx>
	  of the function <m>f(x)</m> if <m>g(x) = cf(x)</m> or <m>g = \frac{1}{c}f(x)</m>.
	</p>
	<ul>
	  <li>
	    <p>
	      The graph of <m>g(x) = cf(x)</m> is obtained by stretching the graph of <m>y = f(x)</m> vertically by a factor of <m>c</m>.
	    </p>
	  </li>
	  <li>
	    <p>
	      The graph of <m>g(x) = \frac{1}{c}f(x)</m> is obtained by compressing the graph of <m>y = f(x)</m> vertically by a factor of <m>c</m>.
	    </p>
	  </li>
	</ul>
      </definition>

      <example>
	<statement>
	  <p>
	    Use <xref ref="fig-parabola" text="title"/> to graph the functions <m>g(x) = 2x^2</m> and <m>h(x) = \frac{2}{3}x^2</m>.
	  </p>
	</statement>
	<solution>
	  <p>
	    The graph of <m>g(x)</m> is obtained by stretching the graph of <m>f(x)</m> vertically by a factor of <m>2</m>, and the graph of <m>h(x)</m> is obtained by compressing the graph the graph of <m>f(x)</m> vertically by a factor of <m>\frac{3}{2}</m>.
	  </p>
	  <figure>
	    <image>
	      <latex-image>
		<xi:include parse="text" href="tex/transformations/vertical_scaling.tex"/>
	      </latex-image>
	    </image>
	  </figure>
	</solution>
      </example>
      
    </subsubsection>

    <subsection>
      <title>Reflection</title>

      <definition xml:id="def-reflection">
	<title>Reflection</title>
	<p>
	  We say the function <m>g(x)</m> is a <term>reflection</term>
	  <idx>
	    <h>Graph</h>
	    <h>Tranformation</h>
	    <h>Reflection</h>
	  </idx>
	  of <m>f(x)</m> if either <m>g(x) = -f(x)</m> or <m>g(x) = f(-x).</m>
	</p>
	<ul>
	  <li>
	    <p>
	      The graph of <m>g(x) = -f(x)</m> is obtained by reflecting the graph of <m>y = f(x)</m> over the <m>x</m>-axis.
	    </p>
	  </li>
	  <li>
	    <p>
	      The graph of <m>g(x) = f(-x)</m> is obtained by reflecting the graph of <m>y = f(x)</m> over the <m>y</m>-axis.
	    </p>
	  </li>
	</ul>
      </definition>

      <example>
	<statement>
	  <p>
	    Use <xref ref="fig-sq_root" text="title"/> to graph the functions <m>g(x) = -\sqrt{x}</m> and <m>h(x) = \sqrt{-x}</m>.
	  </p>
	</statement>
	<solution>
	  <p>
	    The graph of <m>g(x)</m> is obtained by reflecting the graph of <m>f(x)</m> over the <m>x</m>-axis, and the graph of <m>h(x)</m> is obtained by reflecting the graph of <m>f(x)</m> over the <m>y</m>-axis.
	  </p>
	  <figure>
	    <image>
	      <latex-image>
		<xi:include parse="text" href="tex/transformations/reflections.tex"/>
	      </latex-image>
	    </image>
	  </figure>
	</solution>
      </example>
    </subsection>
    
    <subsubsection>
      <title>Horizontal Scaling</title>

      <definition xml:id="def-horizontal_scaling">
	<title>Horizontal Scaling</title>
	<p>
	  Let <m>c > 1</m> be a number.
	  We say the function <m>g(x)</m> is a <term>horizontal scaling</term>
	  <idx>
	    <h>Graph</h>
	    <h>Tranformation</h>
	    <h>Scaling</h>
	    <h>Horizontal</h>
	  </idx>
	  of the function <m>f(x)</m> if <m>g(x) = f(cx)</m> or <m>g(x) = f\left(\frac{1}{c}x\right)</m>.
	</p>
	<ul>
	  <li>
	    <p>
	      The graph of <m>g(x) = f(cx)</m> is obtained by compressing the graph of <m>y = f(x)</m> horizontally by a factor of <m>c</m>.
	    </p>
	  </li>
	  <li>
	    <p>
	      The graph of <m>g(x) = f\left(\frac{1}{c}x\right)</m> is obtained by stretching the graph of <m>y = f(x)</m> horizontally by a factor of <m>c</m>.
	    </p>
	  </li>
	</ul>
      </definition>

      <example>
	<statement>
	  <p>
	    Use <xref ref="fig-parabola" text="title"/> to graph the functions <m>g(x) = (2x)^2</m> and <m>h(x) = \left(\frac{2}{3}x\right)^2</m>.
	  </p>
	</statement>
	<solution>
	  <p>
	    The graph of <m>g(x)</m> is obtained by compressing the graph of <m>f(x)</m> horizontally by a factor of <m>2</m>, and the graph of <m>h(x)</m> is obtained by stretching the graph of <m>f(x)</m> horizontally by a factor of <m>\frac{3}{2}</m>.
	  </p>
	  <figure>
	    <image>
	      <latex-image>
		<xi:include parse="text" href="tex/transformations/horizontal_scaling.tex"/>
	      </latex-image>
	    </image>
	  </figure>
	</solution>
      </example>
    </subsubsection>

    <subsubsection>
      <title>Combining Graph Transformations</title>

      <p>
	Most functions are obtained from a basic function using multiple transformations.
	When graphing a function, the order in which transformations are applied is important.
      </p>
      <algorithm>
	<title>Graphing Functions using Transformations</title>
	<ol>
	  <li>Horizontal Translation</li>
	  <li>Scaling</li>
	  <li>Reflection</li>
	  <li>Vertical Translation</li>
	</ol>
      </algorithm>

      <example>
	<statement>
	  <p>
	    Use <xref ref="fig-parabola" text="title"/> to graph the function <m>g(x) = 2(x + 3)^2 - 2</m>.
	  </p>
	</statement>
	<solution>
	  <p>
	    We can graph <m>g(x)</m> by starting from the basic function <m>f(x) = x^2</m> and applying the following transformations:
	    <ol>
	      <li>Translate the graph of <m>f(x) = x^2</m> to the left by 3 to obtain the graph of <m>(x+3)^2</m>.</li>
	      <li>Stretch the graph of <m>(x+3)^2</m> vertically by a factor of 2 to obtain the graph of <m>2(x+3)^2</m>.</li>
	      <li>Translate the graph of <m>2(x + 3)^2</m> down by 2 units to obtain the graph of <m>g(x) = 2(x + 3)^2 - 2</m>.</li>
	    </ol>
	  </p>
	  <figure>
	    <image>
	      <latex-image>
		<xi:include parse="text" href="tex/transformations/combined.tex"/>
	      </latex-image>
	    </image>
	  </figure>
	</solution>
      </example>
      
    </subsubsection>
  </subsection>

  <worksheet>
    <objectives>
      <introduction>
	<p>Use graphs of basic functions and the following operations to graph general functions.</p>
      </introduction>
      <ul>
	<li>
	  Vertical Translation
	</li>
	<li>
	  Horizontal Translation
	</li>
	<li>
	  Vertical Scaling,
	</li>
	<li>
	  Horizontal Scaling, and
	</li>
	<li>
	  Reflection.
	</li>
      </ul>
    </objectives>
  </worksheet>
</section>


