<?xml version="1.0" encoding="UTF-8"?>

<section xml:id="sec-roots_quadratics" xmlns:xi="http://www.w3.org/2001/XInclude">
  <title>Roots of Quadratic Functions</title>

  <introduction>
    <p>
      In order to accurately graph a quadratic function <m>y = f(x) = ax^2 + bx + c</m>, it is necessary to identify the <m>x</m>-intercepts for the function.
      A point <m>(x,0)</m> in the Cartesian plane is an <xref ref="def-x_intercept" text="title"/> for this function if
      <me>0 = ax^2 + bx + c.</me>
      This reduces the geometric problem of finding the <m>x</m>-intercepts of a quadratic to the algebraic problem finding solutions to equations.
    </p>
  </introduction>
  
  <subsection>
    <title>The Quadratic Formula</title>
    
    <definition>
      <statement>
	<p>
	  An equation of the form <m>ax^2 + bx + c = 0</m> is called a <term>quadratic equation</term>
	  <idx>
	    <h>Equation</h>
	    <h>Quadratic</h>
	  </idx>
	</p>
      </statement>
    </definition>

    <p>
      To find the solutions to the quadratic equation <m>ax^2 + bx + c</m>, we use <xref ref="def-vertex_form" text="title"/> to write 
      <me>0 = ax^2 + bx + c = a\left(x + \frac{b}{2a}\right)^2 - \frac{b^2 - 4ac}{4a}</me>
      and solve this equation for <m>x</m>
      <md>
	<mrow>\amp a\left(x + \frac{b}{2a}\right)^2 - \frac{b^2 - 4ac}{4a} = 0 \amp\amp \text{Add}\ \frac{b^2 - 4ac}{4a}\ \text{to both sides}</mrow>
	<mrow>\amp a\left(x + \frac{b}{2a}\right)^2 = \frac{b^2 - 4ac}{4a} \amp\amp \text{Divide both sides by}\ a</mrow>
	<mrow>\amp \left(x + \frac{b}{2a}\right)^2 = \frac{b^2 - 4ac}{4a^2} \amp\amp \text{Take the square root of both sides}</mrow>
	<mrow>\amp x + \frac{b}{2a} = \pm\sqrt{\frac{b^2 - 4ac}{4a^2}} \amp\amp \text{Simplify}</mrow>
	<mrow>\amp x + \frac{b}{2a} = \pm\frac{\sqrt{b^2 - 4ac}}{\sqrt{4a^2}} \amp\amp \text{Simplify}</mrow>
	<mrow>\amp x + \frac{b}{2a} = \frac{\sqrt{b^2 - 4ac}}{2a} \amp\amp \text{Subtract}\ \frac{b}{2a}\ \text{from both sides}</mrow>
	<mrow>\amp x = - \frac{b}{2a} + \frac{\sqrt{b^2 - 4ac}}{2a} \amp\amp \text{Simplify}</mrow>
	<mrow>\amp x = \frac{-b \pm \sqrt{b^2 - 4ac}}{2a} \amp\amp \text{Simplify}</mrow>
      </md>
    </p>

    <p>
      It is important to note that
      <me>x = \frac{-b + \sqrt{b^2 - 4ac}}{2a}
      \quad\text{and}\quad
      x = \frac{-b - \sqrt{b^2 - 4ac}}{2a} 
      </me>
      are real numbers only when <m>b^2 - 4ac</m> is a non-negative number.
      The number <m>b^2 - 4ac</m> is an important invariant of a quadratic function.
    </p>
    
    <definition xml:id="def-discriminant">
      <title>The Discriminant</title>
      <statement>
	<p>
	  The <term>discriminant</term>
	  <idx>
	    <h>Function</h>
	    <h>Quadratic</h>
	    <h>Discriminant</h>
	  </idx>
	  of the quadratic function <m>f(x) = ax^2 + bx + c</m> is the number
	  <me>D = b^2 - 4ac</me>
	</p>
      </statement>
    </definition>

    <p>
      The discriminant provides both algebraic and geometric information about quadratic functions.
      On the algebraic side, the discriminant tells us how many solutions there are to the quadratic equation
      <m>ax^2 + bx  +c = 0</m>.
    </p>

    <claim xml:id="quadratic_formula">
      <title>The Quadratic Formula</title>
      <statement>
	<p>
	  The quadratic equation
	  <me>ax + bx + c = 0</me>
	  has either two, one, or zero real solutions, depending on <xref ref="def-discriminant" text="title"/>, <m>D = b^2 - 4ac</m>.
	  <ol>
	    <li>
	      <p>
		If <m>D > 0</m>, then the two solutions are
		<me>x = \frac{-b + \sqrt{D}}{2a}
		\quad\text{and}\quad
		x = \frac{-b - \sqrt{D}}{2a}.</me>
	      </p>
	    </li>
	    <li>
	      If <m>D = 0</m>, then the only solution is
	      <me>x = \frac{-b + \sqrt{D}}{2a} = \frac{-b}{2a}.</me>
	    </li>
	    <li>
	      If <m>D \lt 0</m>, then there are no real solutions.
	    </li>
	  </ol>
	</p>
      </statement>
    </claim>

    <p>
      If we pair <xref ref="quadratic_formula" text="title"/> with <xref ref="thm-root_div"/>, then we have an algorithmic way to factor any quadratic function.
    </p>

    <theorem xml:id="thm-quadratic_factorization">
      <statement>
	<p>
	  The quadratic function <m>f(x) = ax^2 + bx + c</m> factors as
	  <me>f(x) = a\left(x - \frac{-b + \sqrt{D}}{2a}\right)\left(x - \frac{-b - \sqrt{D}}{2a}\right),</me>
	  where <m>D = b^2 - 4ac</m> is the <xref ref="def-discriminant" text="title"/>.
	</p>
      </statement>
    </theorem>

    <!-- <example> -->
    <!--   <statement> -->
    <!-- 	<p> -->
    <!-- 	  Factor the quadratic <m>f(x) = -x^2 + 4x + 3</m>. -->
    <!-- 	</p> -->
    <!--   </statement> -->
    <!--   <solution> -->
    <!-- 	<p> -->
    <!-- 	  The discriminant is -->
    <!-- 	  <me>D = 4^2 - 4(-1)(3) = 16 + 12 = 28</me> -->
    <!-- 	  so the roots of <m>f(x)</m> occur at -->
    <!-- 	  <md> -->
    <!-- 	    <mrow>\frac{-4 + \sqrt{28}}{2(-1)} \amp= -\frac{-4 + 2\sqrt{7}}{2} = -(-2 + \sqrt{7}) = 2 - \sqrt{7} ,\,\text{and}</mrow> -->
    <!-- 	    <mrow>\frac{-4 - \sqrt{28}}{2(-1)} \amp= -\frac{-4 - 2\sqrt{7}}{2} = -(-2 - \sqrt{7}) = 2 + \sqrt{7}.</mrow> -->
    <!-- 	  </md> -->
    <!-- 	  We can check this yields the factorization -->
    <!-- 	  <md> -->
    <!-- 	    <mrow>-\left(x - (2 - \sqrt{7})\right)\left(x - (2 + \sqrt{7})\right) -->
    <!-- 	    \amp = -\left(x^2 - (2 + \sqrt{7})x - (2 - \sqrt{7})x + (2 - \sqrt{7})(2 + \sqrt{7})\right) -->
    <!-- 	    </mrow> -->
    <!-- 	    <mrow>\amp = -x^2 + (2 + \sqrt{7} + 2 - \sqrt{7})x - (4 - 7)</mrow> -->
    <!-- 	    <mrow>\amp = -x^2 + 4x + 3 = f(x).</mrow> -->
    <!-- 	  </md> -->
    <!-- 	</p> -->
    <!--   </solution> -->
    <!-- </example> -->

    <example component="web">
      <statement>
	<p>
	  Factor the quadratic <m>f(x) = 10x^2 - 11x + 3</m>.
	</p>
      </statement>
      <solution>
	<p>
	  The discriminant is
	  <me>D = (-11)^2 - 4(10)(3) = 121 - 120 = 1</me>
	  so the roots are
	  <md>
	    <mrow>x \amp= \frac{-(-11) + \sqrt{1}}{2(10)} = \frac{11 + 1}{20} = \frac{12}{20} = \frac{3}{5},\,\text{and}</mrow>
	    <mrow>x \amp = \frac{-(-11) - \sqrt{1}}{2(10)} = \frac{11 - 1}{20} = \frac{10}{20} = \frac{1}{2}.</mrow>
	  </md>
	  By <xref ref="thm-quadratic_factorization"/>, the factorization is
	  <me>10\left(x - \frac{1}{2}\right)\left(x - \frac{3}{5}\right)
	  = 2\left(x - \frac{1}{2}\right)5\left(x - \frac{3}{5}\right)
	  = (2x - 1)(5x - 3).</me>
	  We can check our answer by using FOIL to see
	  <me>(2x - 1)(5x - 3) = 10x^2 - 6x - 5x + 3 = 10x^2 -11x + 3 = f(x).</me>
	</p>
      </solution>
    </example>

    <worksheet component="notes">
      <title/>
      <example>
	<task workspace="4in">
	  <statement>
	    <p>
	      Find the roots of the quadratic function <m>f(x) = 10x^2 - 11x + 3</m>.
	    </p>
	  </statement>
	</task>

	<task workspace="4in">
	  <statement>
	    <p>
	      Use the roots of the quadratic function to factor <m>f</m> into the product of two linear polynomials.
	    </p>
	  </statement>
	</task>
      </example>
    </worksheet>
    
    
    <p>
      On the geometric side, the discriminant tells us how many <m>x</m>-intercepts the graph of <m>y = ax^2 + bx + c</m> has.
    </p>
    
    <theorem>
      <title>The <m>x</m>-intercepts of a Quadratic Function</title>
      <statement>
	<p>
	  The quadratic function <m>y = ax^2 + bx + c</m> has either two, one, or zero <m>x</m>-intercepts, depending on the <xref ref="def-discriminant" text="title"/>, <m>D = b^2 - 4ac</m>.
	  <ol>
	    <li>
	      <p>
		If <m>D > 0</m>, then there are two <m>x</m>-intercepts,
		<me>\left(\frac{-b + \sqrt{D}}{2a},0\right)
		\quad\text{and}\quad
		\left(\frac{-b - \sqrt{D}}{2a},\right).</me>
	      </p>
	    </li>
	    <li>
	      If <m>D = 0</m>, then there is one <m>x</m>-intercept
	      <me>\left(\frac{-b}{2a},0\right).</me>
	      Note this is the vertex.
	    </li>
	    <li>
	      If <m>D \lt 0</m>, then there are no <m>x</m>-intercepts.
	    </li>
	  </ol>
	</p>
      </statement>
    </theorem>

    <example component="web">
      <statement>
	<p>
	  Find the <m>x</m>-intercepts of the function <m>f(x) = 3x^2 + 2x + 4</m>.
	</p>
      </statement>
      <solution>
	<p>
	  Since the discriminant is
	  <me>D = 2^2 - 4(3)(4) = 4 - 48 = -44 \lt 0,</me>
	  this function does not have any <m>x</m>-intercepts.
	</p>
      </solution>
    </example>

    <example component="web">
      <statement>
	<p>
	  Find the <m>x</m>-intercepts of the function <m>f(x) = -3x^2 - 5x + 2</m>.
	</p>
      </statement>
      <solution>
	<p>
	  The discriminant of this quadratic is
	  <me>D = (-5)^2 - 4(-3)(2) = 25 + 24 = 49 = 7^2.</me>
	  The solutions to the equation <m>-3x^2 - 5x + 2 = 0</m> are given by the formula
	  <me>x = \frac{-b \pm \sqrt{D}}{2a}
	  = \frac{-(-5) \pm \sqrt{7^2}}{2(-3)}
	  = \frac{5 \pm 7}{-6}</me>
	  This tells us that one intercept occurs when
	  <me>x = \frac{5 + 7}{-6} = - \frac{12}{6} = -2</me>
	  and the other occurs when
	  <me>x = \frac{5 - 7}{-6} = \frac{-2}{-6} = \frac{1}{3}.</me>
	  Therefore the <m>x</m>-intercepts are
	  <me>\left(-2,0\right) \quad\text{and}\quad \left(\frac{1}{3},0\right).</me>
	</p>
      </solution>
    </example>

    <worksheet component="notes">
      <title/>
      <example>
	<task workspace="4in">
	  <statement>
	    <p>
	      Find the <m>x</m>-intercepts of the function <m>f(x) = 3x^2 + 2x + 4</m>.
	    </p>
	  </statement>
	</task>

	<task workspace="4in">
	  <statement>
	    <p>
	      Find the <m>x</m>-intercepts of the function <m>f(x) = -3x^2 - 5x + 2</m>.
	    </p>
	  </statement>
	</task>
      </example>
    </worksheet>
</subsection>


<subsection>
  <title>Graphing Quadratics</title>

  <p>
    We can simplify the process of graphing a quadratic function by using the tools we have developed in this section.
  </p>
  
  <algorithm>
    <title>Graphing a Quadratic Function</title>
    <statement>
      <p>
	<ol>
	  <li>
	    <p>
	      Use the <xref ref="vertex_formula" text="title"/> to find the vertex, <m>(h,k)</m>, of the parabola.
	      Plot the vertex in the plane.
	    </p>
	  </li>
	  <li>
	    <p>
	      Factor or use the <xref ref="quadratic_formula" text="title"/> to find the <m>x</m>-intercept(s).
	      If there are <m>x</m>-intercepts, plot them in the plane.
	    </p>
	  </li>
	  <li>
	    <p>
	      Plot the <m>y</m>-intercept, <m>(0, f(0))</m>, in the plane.
	    </p>
	  </li>
	  <li>
	    <p>
	      Draw a parabola through the points in Steps (1) through (3).
	      <ul>
		<li>
		  The parabola will open upwards if <m>0 \lt a</m>.
		</li>
		<li>
		  The parabola will open downwards if <m>a \lt 0</m>.
		</li>
	      </ul>
	    </p>
	  </li>
	</ol>
      </p>
    </statement>
  </algorithm>
</subsection>

<xi:include href="worksheets/wksht-roots_quadratics.ptx"/>

<exercises component="web">
  <introduction>
    <p>
      Sketch a graph of each of the quadratic functions below.
      Label the <m>y</m>-intercept, the vertex, and any <m>x</m>-intercepts.
    </p>
  </introduction>

  <exercise>
    <statement>
      <p>
	<m>f(x) = x^2 - 5x + 6</m>
      </p>
    </statement>
  </exercise>

  <exercise>
    <statement>
      <p>
	<m>g(x) = 2x^2 + 4x - 3</m>
      </p>
    </statement>
  </exercise>
  
  <exercise>
    <statement>
      <p>
	<m>h(x) = -8x^2 + 10x + 5</m>
      </p>
    </statement>
  </exercise>

  <exercise>
    <statement>
      <p>
	<m>k(x) = x^2 + x + 1</m>
      </p>
    </statement>
  </exercise>
  
  <exercise>
    <statement>
      <p>
	<m>p(x) = x^2 - 3x - 4</m>
      </p>
    </statement>
  </exercise>

  <exercise>
    <statement>
      <p>
	<m>q(x) = -2x^2 + 6x - 5</m>
      </p>
    </statement>
  </exercise>
</exercises>
</section>
