<?xml version="1.0" encoding="UTF-8"?>

<section xml:id="sec-circles" xmlns:xi="http://www.w3.org/2001/XInclude">
  <title>Circles</title>
  <objectives>
    <ul>
      <li>
	Complete the square to put the equation of a circle into standard form.
      </li>
      <li>
	Use the standard form of a circle to identify the center and radius.
      </li>
      <li>
	Use the standard form of a circle to produce a graph.
      </li>
    </ul>
  </objectives>

  <introduction>
    <p>
      In this section, we study circles in the Cartesian plane.
    </p>

    <definition>
      <p>
	The <term>circle</term>
	<idx>
	  <h>Circle</h>
	</idx>
	with radius <m>r</m> centered at <m>(h,k)</m> consists of all points in the Cartesian plane <m>r</m> units away from <m>(h,k)</m> as depicted in <xref ref="fig-circle_def"/>.
      </p>
      <figure xml:id="fig-circle_def">
	<caption>The circle of radius <m>r</m> centered at <m>(h,k)</m>.</caption>
	<image xml:id="img-circle_def" width="50%">
	  
	  <latex-image>
	    <xi:include parse="text" href="tex/circle_def.tex"/>
	  </latex-image>
	</image>
      </figure>
    </definition>
    
    <p>
      To find the equation of the circle with radius <m>r</m> and center <m>(h,k)</m> we use <xref ref="def-2_distance" text="title"/>.
      A point <m>(x,y)</m> is on this circle if the distance between <m>(x,y)</m> and <m>(h,k)</m> is exactly <m>r</m>:
      <me>
	r = \sqrt{(x - h)^2 + (y - k)^2}.
      </me>
      To make this simpler, we square each side of the equation.
    </p>

    <definition>
      <title>The Standard Form of a Circle</title>
      <p>
	The <term>standard form of a circle</term>
	<idx>
	  <h>Equation</h>
	  <h>Circle</h>
	  <h>Standard Form</h>
	</idx>
	with radius <m>r</m> and center <m>(h,k)</m> is
	<me>
	  (x - h)^2 + (y - k)^2 = r^2.
	</me>
      </p>
    </definition>

    <definition>
      <p>
	A <term>diameter</term>
	<idx>
	  <h>Circle</h>
	  <h>Diameter</h>
	</idx>
	of a circle is a line that connects two points on the circle through the center.
	The length of a diameter of a circle of radius <m>r</m> is <m>2r</m>, and the midpoint of the diameter is the center of the circle.
      </p>
      <figure xml:id="fig-diameter">
	<caption>A diameter of the circle of radius <m>r</m> centered at <m>(h,k)</m>.</caption>
	<image xml:id="img-diameter" width="50%">
	  <latex-image>
	    <xi:include parse="text" href="tex/diameter.tex"/>
	  </latex-image>
	</image>
      </figure>
    </definition>
  </introduction>

  <subsection xml:id="subsec-completing_the_square">
    <title>Completing the Square</title>
    <p>
      Remember that when we multiply two binomials, we must distribute.
      We can remember how to distribute using the mnemonic FOIL: <alert>F</alert>irst, <alert>O</alert>uter, <alert>I</alert>nner, <alert>L</alert>ast:
    </p>
    <figure>
      <caption>How to multiply binomials using the FOIL method.</caption>
      <image source="images/FOIL.png"/>
    </figure>
    <p>
      We can use this method to multiply a binomial by itself
      <md>
	<mrow>
	  (x + a)^2 \amp = (x + a)(x + a)
	</mrow>
	<mrow>\amp = xx + xa + ax + aa</mrow>
	<mrow>\amp = x^2 + ax + ax + a^2</mrow>
	<mrow>\amp = x^2 + 2ax + a^2.</mrow>
      </md>
      We call a trinomial of the form <m>x^2 + 2ax + a^2</m> a <term>perfect square</term>.
      <idx>
	<h>Perfect Square</h>
      </idx>
    </p>
    <p>
      If we have a trinomial of the form <m>ax^2 + bx + c</m>, then we can use the formula
      <me>(x + a)^2 = x^2 + 2ax + a^2 </me>
      to <term>complete the square</term>
      <idx>
	<h>Complete the Square</h>
      </idx>
      as follows.
      <algorithm xml:id="alg-completing_the_square">
	<title>Completing the Square</title>
	<ol>
	  <li>
	    Factor an <m>a</m> from the first two terms to get
	    <me>ax^2 + bx + c = a\left(x^2 + \frac{b}{a}x\right) + c.</me>
	  </li>
	  <li>
	    Add and subtract <m>\left(\frac{b}{2a}\right)^2</m> inside the parentheses to get
	    <me>
	      ax^2 + bx + c = a\left(x^2 + \frac{b}{a}x + \left(\frac{b}{2a}\right)^2 - \left(\frac{b}{2a}\right)^2 \right) + c
	    </me>
	  </li>
	  <li>
	    Recognize the first three terms inside the parentheses as a perfect square
	    <me>ax^2 + bx + c = a\left(\left(x + \frac{b}{2a}\right)^2 - \left(\frac{b}{2a}\right)^2 \right) + c</me>
	  </li>
	  <li>
	    Distribute the <m>a</m> in front through the sum to get
	    <md>
	      <mrow>ax^2 + bx + c \amp= a\left(x + \frac{b}{2a}\right)^2 - a\left(\frac{b}{2a}\right)^2 + c</mrow>
	    </md>
	  </li>
	</ol>
      </algorithm>
    </p>

    <example>
      <statement>
	<p>
	  Complete the square with <m>x^2 + 4x + 5</m>.
	</p>
      </statement>
      <solution>
	<p> When the coefficient on <m>x^2</m> is 1, we can skip the first step and the last step:</p>
	<md>
	  <mrow>x^2 + 4x + 5 \amp= x^2 + 4x + 2^2 - 2^2 + 5 \amp\amp \text{Add and subtract}\ \left(\frac{4}{2}\right)^2 = 2^2 = 4</mrow>
	  <mrow>\amp = (x + 2)^2 - 4 + 5 \amp\amp \text{Factor}</mrow>
	  <mrow>\amp = (x + 2)^2 + 1 \amp\amp \text{Simplify}.</mrow>
	</md>
      </solution>
    </example>
    <example>
      <statement>
	<p>
	  Complete the square with <m>3x^2 - 4x + 5</m>.
	</p>
      </statement>
      <solution>
      <p>
	When the coefficient on <m>x</m> is a negative number, such as <m>x^2 - 4x + 5</m>, we can still use the formula by rewriting the subtraction as addition with a negative number.
	<md>
	  <mrow>3x^2 - 4x + 5 \amp = 3x^2 + (-4)x + 5 \amp\amp \text{Factor}\ 3\ \text{from the first two terms}</mrow>
	  <mrow>\amp= 3\left(x^2 + \left(-\frac{4}{3}\right)x\right) + 5 \amp\amp \text{Add and subtract}\ \left(\frac{\frac{4}{3}}{2}\right)^2 = \left(\frac{2}{3}\right)^2</mrow>
	  <mrow>\amp = 3\left(x^2 + \left(-\frac{4}{3}\right)x +  \left(-\frac{2}{3}\right)^2 - \left(-\frac{2}{3}\right)^2\right) + 5 \amp\amp \text{Factor}</mrow>
	  <mrow>\amp = 3\left(\left(x + \left(-\frac{2}{3}\right)\right)^2 - \frac{4}{9}\right) + 5 \amp\amp \text{Distribute}</mrow>
	  <mrow>\amp = 3\left(x - \frac{2}{3}\right)^2 - \frac{4}{3} + \frac{15}{3} \amp\amp \text{Simplify}</mrow>
	  <mrow>\amp = 3\left(x - \frac{2}{3}\right)^2 + \frac{11}{3}.</mrow>
	</md>
      </p>
      </solution>
    </example>
  </subsection>

  <subsection>
    <title>Recognizing Circles</title>
    <p>
      Sometimes, we will encounter the equation of a circle that is not in standard form.
      We can use <xref ref="alg-completing_the_square" text="title"/> twice to put it back into standard form.
      For example, consider the equation
      <m>x^2 - 4x + y^2 + 6x = -9.</m>
      While this does not look like a circle, we can first complete the square in <m>x</m> as follows.
      First, recognize <m>x^2 - 4x = x^2 + (-4)x</m>.
      Add <m>(-2)^2 = 4</m> to both sides of the equation to obtain
      <me>x^2 + (-4)x + (-2)^2 + y^2 + 6x = -9 + (-2)^2.</me>
      Rewrite the first three terms as a perfect square to obtain
      <me>(x - 2)^2 + y^2 + 6x = -5.</me>
      Next, we complete the square in <m>y</m>.
      Adding <m>3^2 = 9</m> to both sides yields
      <me>(x - 2)^2 + y^2 + 6x + 3^2 = -5 + 9.</me>
      Recognize the trinomial as a perfect square to find
      <me>(x - 2)^2 + (y + 3)^2 = 4.</me>
      Finally, rewrite <m>y + 3</m> as <m>y - (-3)</m> and <m>4 = 2^2</m> to arrive at the standard form of the circle
      <me>(x - 2)^2 + (y - (-3))^2 = 2^2.</me>
      Since these operations preserve the solutions to our equation, we can see that the equation <m>x^2 - 4x + y^2 + 6x = -9</m> represents the circle of radius <m>2</m> centered at the point <m>(2, -3)</m>.
    </p>
    <xi:include href="worksheets/wksht-circles.ptx"/>
  </subsection>
</section>
