<?xml version="1.0" encoding="UTF-8"?>

<section xml:id="sec-inverses" xmlns:xi="http://www.w3.org/2001/XInclude">
  <title>Composition Inverses</title>
  <introduction xml:id="inverses-intro">
    <p>
      In keeping with the analogy with operations on numbers, recall the operations of addition and multiplication both have distinguished elements.
      The number <m>0</m> is called the <term>additive identity</term>
      <idx>
	<h>Identity</h>
	<h>Additive</h>
      </idx>
      because every real number <m>x</m> remains unchanged when <m>0</m> is added to it
      <me>x + 0 = x \quad\text{and}\quad 0 + x = x.</me>
    </p>
    <p>
      Similarly, the number <m>1</m> is called the <term>multiplicative identity</term>
      <idx>
	<h>Identity</h>
	<h>Multiplicative</h>
      </idx>
      because every real number <m>x</m> remains unchanged when it is multiplied by <m>1</m>
      <me>x \times 1 = x \quad\text{and}\quad 1 \times x = x.</me>
    </p>
  </introduction>

  <subsection xml:id="subsec-identities">
    <title>Identities</title>
    <p>
      We introduced the idea of an <em>identity</em> using two familiar operations to highlight that the <alert>identity element depends on the operation.</alert>
      However, the essential <em>behavior</em> of the identity element is the same: when we perform the operation using the identity, nothing changes.
      This tells us exactly how the identity element for the function composition operation should behave.
    </p>

    <definition>
      <title>Identity Function</title>
      <statement>
	<p>
	  Assume <m>A</m> is a set.
	  The <term>identity function</term> on <m>A</m> is the function <m>\id \colon A \to A</m> defined by
	  <me>\id_A(x) = x.</me>
	</p>
      </statement>
    </definition>
    
    <p>
      As we have already seen, the order of function composition matters.
      Complicating matters more, not all functions can be composed.
      For a function <m>f \colon A \to B</m>,
      <ul>
	<li>
	  <p>
	    the composition <m>g \circ f</m> only makes sense when the domain of <m>g</m> contains the range of <m>f</m>, and
	  </p>
	</li>
	<li>
	  <p>
	    the composition <m>f \circ g</m> only makes sense when the range of <m>g</m> is contained in the domain of <m>f</m>.
	  </p>
	</li>
      </ul>
      For this reason, there is not one single identity function that satisfies the condition <m>f \circ \id = f</m> and <m>\id \circ f = f</m>.
    </p>
    <p>
      Instead, we need to consider the identity functions on the domain and codomain of <m>f</m>.
      The identity function on <m>A</m> satisfies <m>f \circ \id_A = f</m> because
      <me>(f \circ \id_A)(x) = f\left(\id_A(x)\right) = f(x)</me>
      and the identity function on <m>B</m> satisfies <m>\id_B \circ f = f</m> because
      <me>(\id_B \circ f)(x) = \id_B\left(f(x)\right) = f(x)</me>.
    </p>
  </subsection>

  <subsection xml:id="subsec-comp_inverses">
    <title>Composition Inverses</title>
    <p>
      The identity elements for these operations are important because they provide a method for "undoing" the operation.
      This is easiest to understand by considering addition and multiplication first.
      For any real number <m>c</m>, the <term>additive inverse</term>
      <idx>
	<h>Inverse</h>
	<h>Additive</h>
      </idx>
      is the real number <m>-c</m> that satisfies
      <me>c + (-c) = 0\quad\text{and}\quad -c + c = 0.</me>
      If we add the number <m>c</m> to another number <m>x</m>, then we obtain the number <m>x + c</m>.
      We can "undo" this operation by performing the operation "add the additive inverse of <m>c</m>" -- which we normally just call "subtract <m>c</m>" -- in the sense that
      <men xml:id="eq-g_of_f">(x + c) + (-c) = x + (c - c) = x + 0 = x.</men>
      Similarly, we note that the operation "add c" will "undo" the operation "subtract <m>c</m>" in the sense that
      <men xml:id="eq-f_of_g">(x - c) + c = x + (-c + c) = x + 0 = x.</men>
    </p>
    <p>
      The operations "add <m>c</m>" and "subtract <m>c</m>" define functions <m>\operatorname{add}_c \colon \R \to \R</m> and <m>\operatorname{add}_{-c} \colon \R \to \R</m> by
      <me>\operatorname{add}_c(x) = x + c \quad\text{and}\quad \operatorname{add}_{-c}(x) = x - c.</me>
      We can view <xref ref="eq-g_of_f"/> and <xref ref="eq-f_of_g"/> in terms of composition:
    </p>
    <sidebyside>
      <p>
	<md>
	  <mrow>\operatorname{add}_{-c} \circ \operatorname{add}_c(x) \amp= \operatorname{add}_{-c}(x + c)</mrow>
	  <mrow>\amp= (x + c) - c </mrow>
	  <mrow>\amp= x</mrow>
	</md>
      </p>
      <p>
	<md>
	  <mrow>\operatorname{add}_c \circ \operatorname{add}_{-c}(x) \amp= \operatorname{add}_c(x - c)</mrow>
	  <mrow>\amp= (x - c) + c </mrow>
	  <mrow>\amp= x.</mrow>
	</md>
      </p>
    </sidebyside>
    <p>
      The story is similar for multiplication.
      For any non-zero real number <m>c</m>, the <term>multiplicative inverse</term>
      <idx>
	<h>Inverse</h>
	<h>Multiplicative</h>
      </idx>
      of <m>c</m> is the real number <m>c^{-1} = 1/c</m> that satisfies
      <me>c \times \frac{1}{c} = 1\quad\text{and}\quad \frac{1}{c} \times c = 1.</me>
      Multiplication by <m>c</m> and multiplication by <m>c^{-1}</m> define functions <m>\operatorname{mul}_c, \operatorname{mul}_{c^{-1}} \colon \R \to \R</m> by
      <me>\operatorname{mul}_c(x) = cx \quad\text{and}\quad \operatorname{mul}_{c^{-1}}(x) = \frac{1}{c}x.</me>
      Just as with addition, these two functions "undo" one another in the sense that
    </p>
    <sidebyside>
      <p>
	<md>
	  <mrow>\operatorname{mul}_c \circ \operatorname{mul}_{c^{-1}}(x) \amp= \operatorname{mul}_c\left(c^{-1}x\right)</mrow><!-- \operatorname{mul}_c\left(\frac{1}{c}x\right)</mrow> -->
	  <mrow>\amp= c\left(\frac{1}{c}x\right) </mrow>
	  <mrow>\amp= x</mrow>
	</md>
      </p>
      <p>
	<md>
	  <mrow>\operatorname{mul}_{c^{-1}} \circ \operatorname{mul}_c(x) \amp= \operatorname{mul}_{c^{-1}}(cx)</mrow>
	  <mrow>\amp= \frac{1}{c}(cx)</mrow>
	  <mrow>\amp= x.</mrow>
	</md>
      </p>
    </sidebyside>
    <p>
      Less formally, one often says "division by <m>c</m>" instead of "multiplication by <m>c^{-1}</m>."
    </p>
    <p>
      These are two canonical examples of functions that are <em>invertible</em>, and the ideas captured in inverting addition and multiplication motivate the more general definition.
    </p>

    <definition xml:id="def-composition_inverse">
      <title>Composition Inverse</title>
      <statement>
	<p>
	  Assume <m>f \colon A \to B</m> is a function.
	  The <term>composition inverse</term>, if it exists, is a function <m>f^{-1} \colon B \to A</m> that satisfies
	  <me>f^{-1} \circ f = \id_A
	  \quad\text{and}\quad
	  f \circ f^{-1} = \id_B
	  </me>
	  or, equivalently, for every <m>x \in A</m>,
	  <m>f^{-1} \circ f(x) = x</m>
	  and for every <m>y \in B</m>,
	  <m>f \circ f^{-1}(y) = y</m>.
	</p>
	<p>
	  If <m>f</m> has a composition inverse, then we say <m>f</m> is <term>invertible</term>.
	  <idx>
	    <h>Function</h>
	    <h>Invertible</h>
	  </idx>
	</p>
      </statement>
    </definition>

    <warning>
      <p>
	Mathematicians commonly use the word "inverse" or "invertible" without explicitly stating the operation.
	It is important to infer the meaning from the context.
	If the object being discussed is a function, then "inverse" means <em>composition</em> inverse, <alert>not</alert> multiplicative inverse.
	That is to say,
	<me>f^{-1}(x) \neq \frac{1}{f(x)} = f(x)^{-1}.</me>
      </p>
      <p>
	In order to avoid confusion, we will avoid using the notation <m>f(x)^{-1}</m> and write either <m>1/f(x)</m> or
	<me>\frac{1}{f(x)}</me>
	whenever we refer to a fraction with the function <m>f(x)</m> in the denominator.
      </p>
    </warning>
  </subsection>

  <subsection xml:id="subsec-props_invertible">
    <title>Properties of Invertible Functions</title>
    <p>
      For a function <m>f \colon A \to B</m> with a composition inverse, the codomain of <m>f</m> and the domain of <m>f^{-1}</m> agree.
      For every <m>y \in B</m>, the element <m>x = f^{-1}(y) \in A</m> satisfies
      <me>y = f \circ f^{-1}(y) = f(x)</me>
      by definition.
      This provides useful information about the range of an invertible function <m>f</m>.
    </p>

    <theorem xml:id="thm-invertible_is_surjective">
      <statement>
	<p>
	  If <m>f \colon A \to B</m> is a function with a composition inverse, then the range of <m>f</m> is <m>f(A) = B.</m>
	</p>
      </statement>
    </theorem>

    <p>
      The definition of a composition inverse is <em>symmetric</em> in the sense that the inverse of <m>f</m> is <m>f^{-1}</m> and the inverse of <m>f^{-1}</m> is <m>f</m>.
    </p>

    <theorem>
      <statement>
	<p>
	  If <m>f \colon A \to B</m> is a function with inverse <m>f^{-1} \colon B \to A</m>, then <m>f^{-1}</m> has a composition inverse and
	  <me>\left(f^{-1}\right)^{-1} = f.</me>
	</p>
      </statement>
    </theorem>
    
    <example xml:id="example-inverse_of_arithmetics">
      <p>
	In the language of <xref ref="def-composition_inverse"/>, the functions "add <m>c</m>" and "add <m>-c</m>" (or "subtract <m>c</m>") are a pair of inverse functions
	<me>\left(\operatorname{add}_{c}\right)^{-1} = \operatorname{add}_{-c}
	\quad\text{and}\quad
	\left(\operatorname{add}_{-c}\right)^{-1} = \operatorname{add}_c.</me>
      </p>
      <p>
	Similarly, the functions "multiply by <m>c</m>" and "multiply by <m>c^{-1}</m>" (or "divide by <m>c</m>") are a pair of inverse functions
	<me>\left(\operatorname{mul}_c\right)^{-1} = \operatorname{mul}_{c^{-1}}
	\quad\text{and}\quad
	\left(\operatorname{mul}_{c^{-1}}\right)^{-1} = \operatorname{mul}_c.</me>
      </p>
    </example>

    <example xml:id="example-inverse_of_composition">
      <p>
	In general, a linear function <m>f(x) = mx + b</m> is invertible if <m>m \neq 0</m>.
	To evaluate <m>f</m> at the real number <m>x</m>, we perform the following operations
	<ol>
	  <li>
	    <p>Multiply <m>x</m> by <m>m</m>,</p>
	  </li>
	  <li>
	    <p>Add <m>b</m> to <m>mx</m>.</p>
	  </li>
	</ol>
	This allows us to decompose <m>f</m> as the function "add <m>b</m>" composed with the function "multiply by <m>m</m>"
	<me>f(x) = \operatorname{add}_b \circ \operatorname{mul}_m(x).</me>
      	Since each function is invertible, we can invert <m>f</m> by performing the inverse operations in reverse order, like peeling back the layers of an onion.
      </p>
      <p>
	Write <m>y = mx + b</m> for the result of applying <m>f</m> to <m>x</m>.
	We would invert (or "undo") the operation of applying <m>f</m> to <m>x</m> by performing the operations
	<ol>
	  <li>
	    <p>
	      Subtract <m>b</m> from <m>y</m>
	    </p>
	  </li>
	  <li>
	    <p>
	      Divide <m>y - b</m> by <m>m</m> (<alert>Important:</alert> This is why we required <m>m \neq 0</m>!)
	    </p>
	  </li>
	</ol>
	Note this is equivalent to solving the equation <m>y = mx + b</m> for <m>x</m> in terms of <m>y</m>
      </p>
      <p>
	In the language of <xref ref="example-inverse_of_arithmetics"/>, the inverse of <m>f</m> is the composition
	<md>
	  <mrow>f^{-1}(y) \amp= \left(\operatorname{mul}_m\right)^{-1} \circ \left(\operatorname{add}_{b}\right)^{-1}(y)</mrow>
	  <mrow>\amp=\operatorname{mul}_{m^{-1}} \circ \operatorname{add}_{-b}(y) </mrow>
	  <mrow>\amp= \operatorname{mul}_{m^{-1}}(y - b)</mrow>
	  <mrow>\amp=\frac{y - b}{m}</mrow>
	  <mrow>\amp=\frac{1}{m}y - \frac{b}{m}.</mrow>
	</md>
      </p>
      <p>
	Finally, we can check these are in fact inverses of one another by checking the two compositions explicitly:
      </p>
      <sidebyside>
	<p>
	  <md>
	    <mrow>f \circ f^{-1}(y) \amp= f\left(\frac{1}{m}y - \frac{b}{m}\right)</mrow>
	    <mrow>\amp= m\left(\frac{1}{m}y - \frac{b}{m}\right) + b</mrow>
	    <mrow>\amp= \frac{m}{m} y - \frac{mb}{m} + b</mrow>
	    <mrow>\amp= y - b + b</mrow>
	    <mrow>\amp=y</mrow>
	  </md>
	</p>
	<p>
	  <md>
	    <mrow>f^{-1} \circ f(x) \amp = f^{-1}(mx + b)</mrow>
	    <mrow>\amp= \frac{1}{m}(mx + b) - \frac{b}{m}</mrow>
	    <mrow>\amp= \frac{m}{m} x + \frac{b}{m} - \frac{b}{m}</mrow>
	    <mrow>\amp= x.</mrow>
	  </md>
	</p>
      </sidebyside>
    </example>
    
    <!-- <example> -->
    <!--   <p> -->
    <!-- 	The linear function <m>f(x) = 3x + 5</m> is an invertible function. -->
    <!-- 	We can find its inverse by solving the equation <m>y = 3x + 5</m> for <m>x</m> in terms of <m>y</m> -->
    <!-- 	<md> -->
    <!-- 	  <mrow>y \amp= 3x + 5 \amp\amp \text{Subtract}\ 5\ \text{from both sides}</mrow> -->
    <!-- 	  <mrow>3x \amp = y - 5 \amp\amp \text{Divide both sides by}\ 3</mrow> -->
    <!-- 	  <mrow>x \amp = \frac{y - 5}{3} \amp\amp\text{Simplify}</mrow> -->
    <!-- 	  <mrow>x \amp = \frac{1}{3}y - \frac{5}{3}.</mrow> -->
    <!-- 	</md> -->
    <!-- 	This tells us the inverse function is -->
    <!-- 	<me>f^{-1}(y) = \frac{1}{3} y - \frac{5}{3}.</me> -->
    <!--   </p> -->
    <!--   <p> -->
    <!-- 	We can verify that these two functions are inverses to one another by computing -->
    <!-- 	<md> -->
    <!-- 	  <mrow>\left(f^{-1} \circ f\right)(x) \amp= f^{-1}\left(3x + 5\right)</mrow> -->
    <!-- 	  <mrow>\amp= \frac{1}{3}\left(3x + 5\right) - \frac{5}{3}</mrow> -->
    <!-- 	  <mrow>\amp= x + \frac{5}{3} - \frac{5}{3}</mrow> -->
    <!-- 	  <mrow>\amp= x</mrow> -->
    <!-- 	</md> -->
    <!-- 	and -->
    <!-- 	<md> -->
    <!-- 	  <mrow>\left(f \circ f^{-1}\right)(y) \amp= f\left(\frac{1}{3}y - \frac{5}{3}\right)</mrow> -->
    <!-- 	  <mrow>\amp= 3\left(\frac{1}{3}y - \frac{5}{3}\right) + 5</mrow> -->
    <!-- 	  <mrow>\amp= y - 5 + 5</mrow> -->
    <!-- 	  <mrow>\amp= y.</mrow> -->
    <!-- 	</md> -->
    <!--   </p> -->
    <!-- </example> -->
    <p>
      Our observations about compositions of invertible functions in <xref ref="example-inverse_of_composition"/> are true in general.
    </p>
    <claim xml:id="formula-inverse_of_composition">
      <statement>
	<p>
	  Assume <m>f</m> and <m>g</m> are invertible functions.
	  If the composition is well-defined, then <m>g \circ f</m> is invertible and
	  <me>\left(g \circ f\right)^{-1} = f^{-1} \circ g^{-1}.</me>
	</p>
      </statement>
    </claim>

    <p>
      As a final example, we illustrate why it is necessary to pay close attention to the domain of a function.
    </p>

    <example xml:id="example-parabola_not_invertible">
      <p>
	Consider the quadratic function <m>f \colon \R \to [0,\infty)</m> defined by <m>f(x) = x^2</m>.
	This function is <alert>not invertible</alert> .
      </p>
      <p>
	To see why, we must observe that if an inverse function exists, then by <xref ref="def-composition_inverse"/>, it must have the form <m>f^{-1} \colon [0,\infty) \to \R</m> and for every positive number <m>y</m>, we must assign a single number <m>x = f^{-1}(y)</m> such that
	<me>x^2 = f(x) = f \circ f^{-1}(y) = y.</me>
      </p>
      <p>
	However, there are always <alert>two</alert> such values: a positive number <m>x</m> and its negative <m>-x</m>.
	This means we must <em>choose</em> one of these two values to be <m>f^{-1}(y)</m>.
	Unfortunately, both decisions fail to produce an inverse for <m>f</m>.
      </p>
      <p>
	If we decide that <m>x = f^{-1}(y)</m> is the positive number such that <m>x^2 = y</m>, then 
	<md>
	  <mrow>f^{-1} \circ f(-x) \amp= f^{-1}\left(\left(-x\right)^2\right)</mrow>
	  <mrow>\amp= f^{-1}(x^2)</mrow>
	  <mrow>\amp= f^{-1}(y)</mrow>
	  <mrow>\amp= x \neq -x.</mrow>
	</md>
      </p>
      <p>
	On the other hand, if we decide that <m>-x = f^{-1}(y)</m> is the negative number such that <m>(-x)^2 = x^2 = y</m>, then
	<me>f^{-1} \circ f(x) = f^{-1}(x^2) = -x \neq x.</me>
	Fortunately, these two problems suggest simple solutions.
      </p>
      <p>
	In the first case, we simply exclude the negative numbers from the domain of <m>f</m>.
	This operation is called <term>restriction</term>
	<idx>
	  <h>Function</h>
	  <h>Restriction</h>
	</idx>
	and produces a new function <m>g \colon [0,\infty) \to [0,\infty)</m> defined by <m>g(x) = x^2</m>.
	This function becomes invertible and its inverse is the <term>principle square root function</term>
	<idx>
	  <h>Function</h>
	  <h>Square Root</h>
	</idx>
	<m>g^{-1} \colon [0,\infty) \to [0,\infty)</m> defined by <m>g^{-1}(y) = \sqrt{y}</m>.
	For every non-negative number <m>x</m>,
      </p>
      <sidebyside>
	<p>
	  <md>
	    <mrow>g^{-1} \circ g(x) \amp= g^{-1}(x^2)</mrow>
	    <mrow>\amp= \sqrt{x^2}</mrow>
	    <mrow>\amp= \abs{x}</mrow>
	    <mrow>\amp= x,</mrow>
	  </md>
	</p>
	<p>
	  <md>
	    <mrow>g \circ g^{-1}(x) \amp= g(\sqrt{x})</mrow>
	    <mrow>\amp= \sqrt{x}^2</mrow>
	    <mrow>\amp= x.</mrow>
	  </md>
	</p>
      </sidebyside>
      <p>
	In the second case, we restrict the domain of <m>f</m> to the negative numbers.
	This produces a new function <m>h \colon (-\infty,0] \to [0,\infty)</m> defined by <m>h(x) = x^2</m>.
	The function <m>h</m> is invertible and its inverse is the function <m>h^{-1} \colon [0,\infty) \to  (-\infty,0]</m> defined by <m>h^{-1}(y) = -\sqrt{y}</m>.
	For every non-negative real number <m>x</m>,
      </p>
      <sidebyside>
	<p>
	  <md>
	    <mrow>h^{-1} \circ h(-x) \amp = h^{-1}\left(\left(-x\right)^2\right)</mrow>
	    <mrow>\amp= h^{-1}(x^2)</mrow>
	    <mrow>\amp= -\sqrt{x^2}</mrow>
	    <mrow>\amp= -\abs{x}</mrow>
	    <mrow>\amp= -x</mrow>
	  </md>
	</p>
	<p>
	  <md>
	    <mrow>h \circ h^{-1}(x) \amp= h\left(-\sqrt{x}\right)</mrow>
	    <mrow>\amp=\left(-\sqrt{x}\right)^2</mrow>
	    <mrow>\amp=(-1)^2\sqrt{x}^2</mrow>
	    <mrow>\amp=\sqrt{x}^2</mrow>
	    <mrow>\amp=x.</mrow>
	  </md>
	</p>
      </sidebyside>
    </example>
  </subsection>

  <xi:include href="./worksheets/wksht-inverses.ptx"/>

  <exercises component="web">
    <introduction>
      <p>
	For each function below, determine a subset of the domain where the function is invertible.
	Find the range of the function on that interval, then find the inverse.
	Indicate the domain and range of the inverse.
      </p>
    </introduction>

    <exercise>
      <statement>
	<p>
	  <m>f(x) = 2x - 3</m>.
	</p>
      </statement>
    </exercise>

    <exercise>
      <statement>
	<p>
	  <m>g(x) = x^2 + 4</m>.
	</p>
      </statement>
    </exercise>

    <exercise>
      <statement>
	<p>
	  <m>h(x) = x^3 - 1</m>.
	</p>
      </statement>
    </exercise>

    <exercise>
      <statement>
	<p>
	  <m>p(x) = \dfrac{2x + 1}{3}</m>.
	</p>
      </statement>
    </exercise>
  </exercises>
</section>
