<?xml version="1.0" encoding="UTF-8"?>

<section xml:id="sec-lines" xmlns:xi="http://www.w3.org/2001/XInclude">
  <title>Representations of Lines</title>
  <objectives>
    <ul>
      <li>
	Determine the slope of a line through two points.
      </li>
      <li>
	<p>
	  Represent a line using
	  <ul>
	    <li>Slope-Intercept Form,</li>
	    <li>Point-Slope Form, and</li>
	    <li>Standard Form.</li>
	  </ul>
	</p>
      </li>
    </ul>
  </objectives>

  <introduction>
    <p>
      In the previous section, we encountered linear functions and saw that we can express these functions in the form <m>y = mx + b</m>.
      When we graphed a linear function, we used to points to determine the line that represents the graph.
      We can reverse this process to find a linear function.
      The first step is to determine the slope.
      In doing this, we will find two other representations for lines.
    </p>
  </introduction>

  <subsection>
    <title>The Slope of a Line through two Points</title> 
    <definition xml:id="def-slope">
    <title>The Slope of a Line</title>
    <p>
      The <term>slope</term>
      <idx>
	<h>Line</h>
	<h>Slope</h>
      </idx>
      of the line through the points <m>(x_1, y_1)</m> and <m>(x_2, y_2)</m> is
      <me>\frac{y_1 - y_2}{x_1 - x_2} = \frac{y_2 - y_1}{x_2 - x_1},</me>
      provided that <m>x_1 \neq x_2</m>.
      The slope measures the rate of change in <m>y</m> with respect to <m>x</m>, as depicted in <xref ref="fig-slope"/>.
    </p>
  </definition>

  <figure xml:id="fig-slope">
    <image xml:id="img-slope">
      <latex-image>
	<xi:include parse="text" href="tex/slope.tex"/>
      </latex-image>
    </image>
    <caption>The slope of the line through the points <m>(x_1, y_1)</m> and <m>(x_2, y_2)</m>.</caption>
  </figure>
  
  <remark>
    <p>
      In the definition of <xref ref="def-slope" text="title"/>, we required that <m>x_1 \neq x_2</m>.
      While there is a line that passes through two distinct points with the same <m>x</m>-coordinate, that line is a vertical line.
      Since a vertical line is <em>not</em> a function, the slope of a vertical line undefined.
    </p>
  </remark>
  
  <example xml:id="example-find_slope">
    <statement>
      <p>Find the slope of the line through the points <m>(3,5)</m> and <m>(6,2)</m>.</p>
    </statement>
    <solution>
      <p>
	The slope of the line through the points <m>(3,5)</m> and <m>(6,2)</m> is
	<me>\frac{2 - 5}{6 - 3} = \frac{-3}{3} = -1.</me>
	This says when the <m>x</m>-coordinate increases by 1, the <m>y</m>-coordinate decreases by 1.
      </p>
    </solution>
  </example>

  <p>
    Suppose we know the slope, <m>m</m>, and a point <m>(x_0, y_0)</m> that lines on the line.
    We can use the fact that <m>(x_0, y_0)</m> is a <xref ref="def-solution" text="title"/> to determine the <m>y</m>-intercept.
    We substitute <m>x_0</m> for <m>x</m> and <m>y_0</m> for <m>y</m> in the <xref ref="thm-slope_intercept" text="title"/> and solve for <m>b</m>:
    <md>
      <mrow>y_0 \amp= mx_0 + b \amp\amp \text{Subtract}\ mx_0\ \text{from both sides}</mrow>
      <mrow>b \amp = y_0 - mx_0.</mrow>
    </md>
  </p>

  <theorem xml:id="thm-point_slope_intercept">
    <statement>
      <p>
	The <m>y</m>-intercept of the line with slope <m>m</m> through the point <m>(x_0, y_0)</m> is
	<me>b = y_0 - mx_0.</me>
      </p>
    </statement>
  </theorem>

  <example xml:id="example-line_through_two_points">
    <statement>
      <p>
	Find the equation of the line through the points <m>(3,5)</m> and <m>(6,2)</m>.
      </p>
    </statement>
    <solution>
      <p>
	In <xref ref="example-find_slope"/>, we saw the slope of the line is <m>-1</m>.
	If we use the point <m>(3,5)</m>, then we can find the <m>y</m>-intercept by solving
	<md>
	  <mrow>5 \amp= -3 + b \amp\amp \text{Add}\ 3\ \text{to both sides}</mrow>
	  <mrow>b \amp= 5 + 3 = 8.</mrow>
	</md>
	This tells us the equation of the line through <m>(3,5)</m> and <m>(6,2)</m> is
	<me>y = -x + 8</me>.
      </p>
      <p>
	We could also have used the point <m>(6,2)</m> to find an equation of the line.
	If we use the point <m>(6,2)</m>, then the <m>y</m>-intercept is given by solving
	<md>
	  <mrow>2 \amp= -6 + b \amp\amp \text{Add}\ 6\ \text{to both sides}</mrow>
	  <mrow>b \amp= 2 + 6 = 8.</mrow>
	</md>
	We can see that no matter which point we use, we obtain the same <xref ref="thm-slope_intercept" text="title"/>.
      </p>
    </solution>
  </example>
  </subsection>

  <subsection>
    <title>The Point-Slope Form of a Line</title>
    
    <p>
      Assume we know the slope, <m>m</m>, of a line and a point, <m>(x_0, y_0)</m>, on the line.
      Suppose <m>(x,y)</m> is any other point on the line.
      Since the slope of the line is constant, we can write
      <md>
	<mrow>m \amp= \frac{y - y_0}{x - x_0} \amp\amp \text{Multiply both sides by}\ x - x_0</mrow>
	<mrow>m(x - x_0) \amp= \left(\frac{y - y_0}{x - x_0}\right)(x - x_0) \amp\amp \text{Simplify}</mrow>
	<mrow>m(x - x_0) \amp = y - y_0 \amp\amp \text{Swap sides}</mrow>
	<mrow>y - y_0 \amp = m(x - x_0)</mrow>
      </md>
      to find the next form of a line.
    </p>
    
    <theorem xml:id="thm-point_slope">
      <title>The Point-Slope Form of a Line</title>
      <statement>
	<p>
	  The <term>point-slope form of the line</term>
	  <idx>
	    <h>Line</h>
	    <h>Point-Slope Form</h>
	  </idx>
	  through the point <m>(x_0, y_0)</m> with slope <m>m</m> is
	  <me>y - y_0 = m(x - x_0).</me>
	</p>    
      </statement>
    </theorem>

    <p>
      This form of a line is convenient to use when we know the slope of a line and a point on the line.
    </p>

    <example>
      <statement>
	<p>
	  Find the <xref ref="thm-point_slope" text="title"/> using the point <m>(1,2)</m> and the slope <m>3</m>.
	</p>
      </statement>
      <solution>
	<p>
	  Using <xref ref="thm-point_slope" text="title"/>, the equation of the line through <m>(1,2)</m> with slope <m>3</m> is
	  <me>y - 2 = 3(x - 1).</me>
	</p>
      </solution>
    </example>

    <example>
      <statement>
	<p>
	  Find an equation for the line that passes through the points <m>(3,2)</m> and <m>(4,3)</m>.
	</p>
      </statement>
      <solution>
	<p>
	  We can use the <xref ref="thm-point_slope" text="title"/> to find the line between the points <m>(3,2)</m> and <m>(4,3)</m>.
	  First compute the slope of the line
	  <me>m = \frac{3 - 2}{4 - 3} = \frac{1}{1} = 1.</me>
	  Use either of the two points to find the equation
	  <me>y - 2 = x - 3
	  \quad\text{or}\quad
	  y - 3 = x - 4.</me>
	</p>
	<p>
	  While these equations may look different, we can compare them by placing them in <xref ref="thm-slope_intercept" text="title"/>.
	  For the first equation, add <m>2</m> to both sides to get
	  <me>y =  x - 1</me>
	  and for the second, add <m>3</m> to both sides to get
	  <me>y = x - 1.</me>
	  In this form, we can see that these equations represent the same line.
	</p>
      </solution>
    </example>
  </subsection>

  <subsection>
    <title>The Standard Equation of a Line</title>
    <p>
      So far, we have only been interested in working with lines with a well-defined slope.
      Sometimes, it is convenient to work with lines that may be vertical.
      The standard equation of a line allows us to do just that.
    </p>

    <definition xml:id="def-linear_equation">
      <title>Standard Equation of a Line</title>
      <p>
        The <term>standard equation of a line</term>
        <idx>
	<h>Equation</h>
	<h>Line</h>
	<h>Standard</h>
        </idx>
        in the variables <m>x</m> and <m>y</m> is
        <me>ax + by = c,</me>
	where <m>a</m> and <m>b</m> are not both zero.
      </p>
    </definition>

    <remark>
      <title><alert>Caution!</alert></title>
      <p>
	The standard equation of a line may not always represent an equation where <m>y</m> is a function of <m>x</m>!
	If <m>b = 0</m>, then the standard equation of a line reduces to
	<md>
	  <mrow>ax \amp= c \amp\amp \text{Divide both sides by}\ a</mrow>
	  <mrow>x \amp = \frac{c}{a},</mrow>
	</md>
	which is a vertical line.
      </p>
    </remark>

    <example>
      <statement>
        <p>
	  Place the linear equation
	  <me>x + 3y - 2x + 7 = 5 + y - 4x</me>
	  into <xref ref="def-linear_equation" text="title" />.
        </p>
      </statement>
      <solution>
        <p>
	  The equation
	  <me>x + 3y - 2x + 7 = 5 + y - 4x</me>
	  can be placed in standard form as follows.
	  First, move the variables to the left-hand side of the equation.
	  Subtract <m>y - 4x</m> from both sides
	  <me>x - 2x + 3y + 7 - (y - 4x) = 5</me>
	  and distribute the negative
	  <me>x - 2x + 3y + 7 - y + 4x = 5.</me>
	  Collect like terms
	  <me>x - 2x + 4x + 3y - y + 7 = 5</me>
	  and simplify
	  <me>3x + 2y + 7 = 5.</me>
	  Finally, subtract 7 from both sides of the equation
	  <me>3x + 4y = 5 - 7</me>
	  and simplify to arrive at the standard form
	  <me>3x + 4y = -2.</me>
        </p>
      </solution>
    </example>

    <example>
      <p>
        Not all equations are linear.
        For example, the equation <m>xy + y - 7 = 2</m> is not linear because of the term <m>xy</m>.
      </p>
    </example>
  </subsection>

  <xi:include href="worksheets/wksht-rep_of_lines.ptx"/>
</section>
