<?xml version="1.0" encoding="UTF-8"?>

<section xml:id="sec-rational_functions" xmlns:xi="http://www.w3.org/2001/XInclude">
  <title>Rational Functions</title>

  <introduction>
    <p>
      A special case of ratios of functions arise when both the numerator and denominator are polynomials.
      These functions are of significant importance in many areas of mathematics, as well as its applications.
    </p>
  </introduction>

  <subsection>
    <title>The Domain of a Rational Function</title>
    <definition xml:id="def-rational_function">
      <statement>
	<p>
	  A <term>rational function</term> is a function of the form
	  <me>f(x) = \left(\frac{p}{q}\right)(x) = \frac{p(x)}{q(x)},</me>
	  where <m>p</m> and <m>q \neq 0</m> are polynomial functions.
	</p>
      </statement>
    </definition>
    <p>
      Since polynomial functions always have domain <m>\R</m> and codomain <m>\R</m>, the domain of the rational function <m>f = p/q</m> is the set
      <me>D = \left\{x \in \R \;\middle\vert\; q(x) \neq 0\right\}.</me>
    </p>
    
    <example component="web">
      <statement>
	<p>
	  Find the domain of the rational function
	  <me>f(x) = \frac{x - 2}{x^2-9}</me>
	</p>
      </statement>
      <solution>
	<p>
	  This expression is undefined whenever 
	  <me>x^2 - 9 = (x - 3)(x + 3) = 0</me>
	  Since the only solutions to this equation are <m>x = 3</m> and <m>x = -3</m>, the domain of <m>f</m> is
	  <me>D = \left\{x \in \R \;\middle\vert\; x \neq \pm 3\right\}.</me>
	  This is the set of all numbers except <m>3</m> and <m>-3</m>, which we can express as the union of intervals
	  <me>(-\infty,-3) \cup (-3, 3) \cup (3, \infty).</me>
	</p>
      </solution>
    </example>

    <worksheet component="notes">
      <title/>
      <page>
	<example>
	  <statement>
	    <p>
	      Find the domain of the rational function
	      <me>f(x) = \frac{x - 2}{x^2-9}</me>
	    </p>
	  </statement>
	</example>
      </page>
    </worksheet>
  </subsection>

  <subsection>
    <title>Simplifying Rational Functions</title>
    <p>
      Recall that we always write rational numbers in lowest terms.
      For example, instead of writing <m>2/4</m>, we cancel the common factor of <m>2</m> in the numerator and denominator to write <m>1/2</m>.
      The same is true for rational functions, although some extra care is required.
    </p>

    <example component="web">
      <statement>
	<p>
	  Simplify the function <m>f \colon (-\infty, 3) \cup (3, \infty) \to \R</m> defined by
	  <me>f(x) = \frac{x^2-9}{x - 3}</me>
	  in lowest terms.
	  What is the domain of this simplified function?
	</p>
      </statement>
      <solution>
	<p>
	  To simplify the expression, factor the numerator as <m>x^2 - 9 = (x - 3)(x + 3)</m> and cancel the common factors in the numerator and denominator
	  <me>f(x) = \frac{x - 3}{x - 3}(x + 3) = x + 3.</me>
	</p>
	<p>
	  It is important to remember that this simplification <alert>only holds for elements of the domain of the function <m>f</m>!</alert>
	  This says that <m>f</m> is equal to the function <m>g \colon (-\infty, 3) \cup (3, \infty) \to \R</m> defined by <m>g(x) = x + 3</m>.
	  However, the function <m>h \colon \R \to \R</m> defined by <m>h(x) = x + 3</m> is <alert>not</alert> equal to the function <m>f</m> because the functions <m>f</m> and <m>h</m> do not have the same domain.
	</p>
      </solution>
    </example>

    <worksheet component="notes">
      <title/>
      <page>
	<example>
	  <statement>
	    <p>
	      Simplify the function <m>f \colon (-\infty, 3) \cup (3, \infty) \to \R</m> defined by
	      <me>f(x) = \frac{x^2-9}{x - 3}</me>
	      in lowest terms.
	      What is the domain of this simplified function?
	    </p>
	  </statement>
	</example>
      </page>
    </worksheet>
  </subsection>

  <subsection>
    <title>Sums and Differences of Rational Functions</title>
    <p>
      Recall that in order to add or subtract rational numbers, we must find a common denominator.
      For example, to add <m>2/3</m> and <m>3/2</m>, we use the common denominator <m>2 \times 3 = 6</m>
      <md>
	<mrow>\frac{2}{3} + \frac{3}{2} \amp= \frac{2}{2}\frac{2}{3} + \frac{3}{3}\frac{3}{2}</mrow>
	<mrow>\amp= \frac{4}{6} + \frac{9}{6}</mrow>
	<mrow>\amp= \frac{4 + 9}{6}</mrow>
	<mrow>\amp= \frac{13}{6}.</mrow>
      </md>
      The same is true for rational functions, provided we are careful with the denominator.
    </p>

    <example component="web">
      <statement>
	<p>
	  Find the sum of the rational functions
	  <me>f \colon \left\{x \in \R \;\middle\vert\; x \neq 0,\, 1\right\} \to \R
	  \quad\text{and}\quad
	  g \colon \left\{x \in \R \;\middle\vert\; x \neq 0,\, 2\right\} \to \R</me>
	  defined by
	  <me>f(x) = \frac{x + 1}{x(x-1)}
	  \quad\text{and}\quad
	  g(x) = \frac{x - 4}{x(x-2)}.</me>
	  What is the domain of this function?
	</p>
      </statement>
      <solution>
	<p>
	  To add these functions, we must first find a common denominator.
	  We use the least common multiple of <m>x(x-1)</m> and <m>x(x-2)</m>, which is
	  <me>x(x - 1)(x - 2).</me>
	  Once we have the common denominator, the process of adding rational functions is nearly the same as for rational numbers:
	  <md>
	    <mrow>\frac{x + 1}{x(x-1)} + \frac{x - 4}{x(x-2)}
	    \amp = \frac{x-2}{x-2}\left(\frac{x + 1}{x(x-1)}\right) + \frac{x-1}{x-1}\left(\frac{x - 4}{x(x-2)}\right)</mrow>
	    <mrow>\amp=\frac{(x-2)(x+1)}{x(x-1)(x-2)} + \frac{(x-1)(x-4)}{x(x-1)(x-2)}</mrow>
	    <mrow>\amp=\frac{(x-2)(x+1) + (x-1)(x-4)}{x(x-1)(x-2)}</mrow>
	    <mrow>\amp=\frac{x^2 +x - 2x - 2 + x^2 - 4x -x + 4}{x(x-1)(x-2)}</mrow>
	    <mrow>\amp=\frac{2x^2 + 1x - 2x -4x -1x -2 + 4}{x(x-1)(x-2)}</mrow>
	    <mrow>\amp=\frac{2x^2 -6x + 2}{x(x-1)(x-2)}.</mrow>
	  </md> 
	</p>
	<p>
	  By <xref ref="def-sum_functions"/>, the function <m>f + g</m> is only defined where <alert>both</alert> of <m>f</m> and <m>g</m> are defined.
	  Therefore the sum of <m>f</m> and <m>g</m> is the function
	  <me>f + g \colon \left\{x \in \R \;\middle\vert\; x \neq 0,\,1,\,2\right\} \to \R</me>
	  defined by
	  <me>(f + g)(x) = \frac{2x^2 -6x + 2}{x(x-1)(x-2)}.</me>
	</p>
      </solution>
    </example>

    <worksheet component="notes">
      <title/>
      <introduction>
	<p>
	  Consider the rational functions
	  <me>f \colon \left\{x \in \R \;\middle\vert\; x \neq 0,\, 1\right\} \to \R
	  \quad\text{and}\quad
	  g \colon \left\{x \in \R \;\middle\vert\; x \neq 0,\, 2\right\} \to \R</me>
	  defined by
	  <me>f(x) = \frac{x + 1}{x(x-1)}
	  \quad\text{and}\quad
	  g(x) = \frac{x - 4}{x(x-2)}.</me>
	</p>
      </introduction>
      <page>
	<example>
	  <statement>
	    <p>
	      Find the sum of <m>f</m> and <m>g</m>.
	      What is the domain of this function?
	    </p>
	  </statement>
	</example>
      </page>
    </worksheet>
    
  </subsection>

  <subsection>
    <title>Products and Ratios of Rational Functions</title>
    <p>
      Recall that when we multiply two rational numbers we multiply the numerators and denominators.
      For example,
      <me>\frac{1}{2}\left(\frac{3}{4}\right) = \frac{1(3)}{2(4)} = \frac{3}{8}.</me>
      When we divide one rational number by another, we multiply the one by the reciprocal of the other.
      For example
      <me>\frac{\frac{1}{2}}{\frac{3}{4}} = \frac{1}{2}\left(\frac{4}{3}\right) = \frac{4}{6} = \frac{2}{3}.</me>
      The same is true for products and ratios of rational functions.
    </p>

    <example component="web">
      <statement>
	<p>
	  Find the product of the rational functions
	  <me>f \colon \left\{x \in \R \;\middle\vert\; x \neq 0,\, 1\right\} \to \R
	  \quad\text{and}\quad
	  g \colon \left\{x \in \R \;\middle\vert\; x \neq 0,\, 2\right\} \to \R</me>
	  defined by
	  <me>f(x) = \frac{x + 1}{x(x-1)}
	  \quad\text{and}\quad
	  g(x) = \frac{x - 4}{x(x-2)}.</me>	
	</p>
      </statement>
      <solution>
	<p>
	  We multiply the rational functions by multiplying the numerators and the denominators
	  <me> \frac{x + 1}{x(x-1)}\left(\frac{x - 4}{x(x-2)}\right)
	  = \frac{(x+1)(x-4)}{x^2(x-1)(x-2)}</me>
	</p>
	<p>
	  By <xref ref="def-product_functions"/>, the function <m>fg</m> is only defined where <alert>both</alert> <m>f</m> and <m>g</m> are defined.
	  Therefore product of <m>f</m> and <m>g</m> is the function
	  <me>fg \colon \left\{x \in \R \;\middle\vert\; x \neq 0, 1, 2\right\} \to \R</me>
	  defined by
	  <me>(fg)(x) = \frac{(x+1)(x-4)}{x^2(x-1)(x-2)}.</me>
	</p>
      </solution>
    </example>

    <example component="web">
      <statement>
	<p>
	  Find the ratio of the rational functions
	  <me>f \colon \left\{x \in \R \;\middle\vert\; x \neq 0,\, 1\right\} \to \R
	  \quad\text{and}\quad
	  g \colon \left\{x \in \R \;\middle\vert\; x \neq 0,\, 2\right\} \to \R</me>
	  defined by
	  <me>f(x) = \frac{x + 1}{x(x-1)}
	  \quad\text{and}\quad
	  g(x) = \frac{x - 4}{x(x-2)}.</me>	
	</p>
      </statement>
      <solution>
	<p>
	  We can divide these rational functions by multiplying <m>f</m> by the reciprocal of <m>g</m>:
	  <md>
	    <mrow>\frac{\frac{x + 1}{x(x-1)}}{\frac{x - 4}{x(x-2)}}
	    \amp= \frac{x + 1}{x(x-1)}\left(\frac{x(x-2)}{x - 4}\right)</mrow>
	    <mrow>\amp= \frac{x(x+1)(x-2)}{x(x-1)(x-4)}</mrow>
	    <mrow>\amp= \frac{(x+1)(x-2)}{(x-1)(x-4)}.</mrow>
	  </md>
	</p>
	<p>
	  By <xref ref="def-ratio_functions"/>, the function <m>f/g</m> is only defined where <alert>both</alert> <m>f</m> and <m>g</m> are defined <alert>and</alert> <m>g</m> is non-zero.
	  Therefore <m>f/g</m> is the function
	  <me>fg \colon \left\{x \in \R \;\middle\vert\; x \neq 0, 1, 2,4\right\} \to \R</me>
	  defined by
	  <me>\left(\frac{f}{g}\right)(x) = \frac{(x+1)(x-2)}{(x-1)(x-4)}.</me>
	</p>
      </solution>
    </example>

    <worksheet component="notes">
      <title/>
      <page>
	<introduction>
	  <p>
	    Consider the rational functions
	    <me>f \colon \left\{x \in \R \;\middle\vert\; x \neq 0,\, 1\right\} \to \R
	    \quad\text{and}\quad
	    g \colon \left\{x \in \R \;\middle\vert\; x \neq 0,\, 2\right\} \to \R</me>
	    defined by
	    <me>f(x) = \frac{x + 1}{x(x-1)}
	    \quad\text{and}\quad
	    g(x) = \frac{x - 4}{x(x-2)}.</me>	
	  </p>
	</introduction>
	<example>
	  <task workspace="4in">
	    <statement>
	    <p>
	      Find the product of <m>f</m> and <m>g</m>.
	    </p>
	  </statement>
	  </task>
	  <task workspace="4in">
	    <statement>
	      <p>
		Find the ratio <m>f</m> and <m>g</m>
	      </p>
	    </statement>
	  </task>
	</example>
      </page>
    </worksheet>
  </subsection>

  <subsection>
    <title>Rational Equations and Inequalities</title>

    <p>
      Just as with polynomials, we may wish to solve equations or inequalities involving rational functions.
      Fortunately, with some care, rational equations and inequalities quickly reduce to polynomial equations or inequalities by simply multiplying both sides by the denominator.
    </p>

    <p>
      Rational inequalities are defined nearly identically to polynomial inequalities.
    </p>
    
    <definition xml:id="def-rational_ineq">
      <title>Rational Inequality</title>
      <statement>
	<p>
	  Assume <m>p \colon \R \to \R</m> and <m>q \colon \R \to \R</m> are polynomial functions.
	  A <term>rational inequality</term>
	  <idx>
	    <h>Inequality</h>
	    <h>Rational</h>
	  </idx>
	  is a relation of the form
	  <ul>
	    <li>
	      <p>
		<m>\frac{p(x)}{q(x)} \lt 0</m>,
	      </p>
	    </li>
	    <li>
	      <p>
		<m>\frac{p(x)}{q(x)} \leq 0</m>,
	      </p>
	    </li>
	    <li>
	      <p>
		<m>\frac{p(x)}{q(x)} > 0</m>, or
	      </p>
	    </li>
	    <li>
	      <p>
		<m>\frac{p(x)}{q(x)} \geq 0</m>.
	      </p>
	    </li>
	  </ul>
	</p>
      </statement>
    </definition>

    <p>
      The solutions are also similarly defined.
    </p>

    <definition xml:id="def-solution_rational_inequality">
      <title>Solution to a Rational Inequality</title>
      <statement>
	<p>
	  A <term>solution</term>
	  <idx>
	    <h>Inequality</h>
	    <h>Solution</h>
	  </idx>
	  to an inequality in the variable <m>x</m> is a number <m>a</m> that makes the expression true when <m>a</m> is substituted for <m>x</m>. 
	</p>
      </statement>
    </definition>

    <example component="web">
      <statement>
	<p>
	  Solve the equation
	  <me>\frac{x^2 - 1}{x^2 - 4} = 3</me>
	</p>
      </statement>
      <solution>
	<p>
	  First we note the domain of the rational function <m>(x^2 - 1)/(x^2 -4)</m> is the set
	  <me>D = \left\{x \in \R \;\middle\vert\; x \neq \pm 2\right\}</me>
	  As long as <m>x \in D</m>, we may multiply both sides of the equation by the non-zero quantity <m>x^2 - 4</m> to obtain the polynomial equation
	  <md>
	    <mrow>\amp x^2 - 1 = 3(x^2 - 4) \amp\amp \text{Distribute}</mrow>
	    <mrow>\amp x^2 - 1 = 3x^2 - 12 \amp\amp \text{Add}\ 12 - x^2\ \text{to both sides}</mrow>
	    <mrow>\amp 11 = 2x^2 \amp\amp \text{Rewrite}</mrow>
	    <mrow>\amp 2x^2 = 11 \amp\amp \text{Divide both sides by}\ 2</mrow>
	    <mrow>\amp x^2 = \frac{11}{2} \amp\amp \text{Take the square root of each side.}</mrow>
	    <mrow>\amp x = \pm \sqrt{\frac{11}{2}}</mrow>
	  </md>
	  Therefore the two solutions are <m>x = \sqrt{11/2}</m> and <m>x = -\sqrt{11/2}.</m>
	</p>
      </solution>
    </example>
    
    <example component="web">
      <statement>
	<p>
	  Solve the rational inequality
	  <me>\frac{x^2 - 1}{x^2 - 4} \leq 3</me>
	</p>
      </statement>
      <solution>
	<p>
	  First, we must place the inequality in the form
	  <me>\frac{p(x)}{q(x)} \leq 3</me>
	  We do this using the operations above
	  <md>
	    <mrow>\amp \frac{x^2 - 1}{x^2 - 4} \leq 3 \amp\amp \text{Subtract}\ 3\ \text{from both sides}</mrow>
	    <mrow>\amp \frac{x^2 - 1}{x^2 - 4} - 3 \leq 0 \amp\amp \text{Find a common denominator}</mrow>
	    <mrow>\amp \frac{x^2 - 1}{x^2 - 4} - \frac{3(x^2 - 4)}{x^2 - 4} \leq 0\amp\amp \text{Combine}</mrow>
	    <mrow>\amp \frac{x^2 - 1 - 3(x^2 - 4)}{x^2 - 4} \leq 0\amp\amp \text{Distribute}</mrow>
	    <mrow>\amp \frac{x^2 - 1 - 3x^2 + 12}{x^2 - 4} \leq 0\amp\amp \text{Simplify}</mrow>
	    <mrow>\amp \frac{-2x^2 + 11}{x^2 - 4} \leq 0</mrow>
	  </md>
	</p>
	<p>
	  Once the inequality is in the proper form, our goal is to reduce from a rational inequality to one or more polynomial inequalities.
	  The tricky part is dealing with the sign of the denominator.
	  We observe that the denominator is positive on the set
	  <me>(-\infty, -2) \cup (2, \infty)</me>
	  and negative on <m>(-2, 2)</m>.
	  Since multiplying both sides of an inequality <alert>reverses the inequality</alert> we must handle these two regions separately.
	</p>
	<p>
	  When <m>x \in (-2, 2)</m>, we obtain the polynomial inequality
	  <md>
	    <mrow>\amp \frac{-2x^2 + 11}{x^2 - 4} \leq 0 \amp\amp \text{Multiply both sides by}\ x^2 - 4</mrow>
	    <mrow>\amp -2x^2 + 11 \geq 0</mrow>
	  </md>
	  The quadratic <m>y = -2x^2 + 11</m> is a downward facing parabola with roots at <m>x = \pm \sqrt{11/2} \approx \pm 2.35</m>.
	  Since
	  <me>-\sqrt{\frac{11}{2}} \lt -2 \lt 2 \lt \sqrt{\frac{11}{2}}</me>
	  it follows that the inequality holds on all of <m>(-2, 2)</m>.
 	</p>
	<figure xml:id="fig-rational_example_case_1">
	  <caption>Solutions to the inequality <m>-2x^2 + 11 \geq 0</m></caption>
	  <image xml:id="img-rational_example_case_1">
	    <latex-image xml:id="tikz-rational_example_case_1">
	      \begin{tikzpicture}[scale=0.5]
	      \def\size{12}
	      
	      \path [draw, help lines, opacity=.5]  (-\size,-\size) grid (\size,\size);
	      
	      \draw [very thick,->] (-\size,0) -- (\size+.1,0) node [anchor=south] {$x$};
	      \draw [very thick,->] (0,-\size) -- (0,\size+.1) node [anchor=west] {$y$};
	      
	      \begin{scope}[domain=-5:5]
	      \clip (-\size,-\size) rectangle (\size,\size);
	      \draw [color=blue,thick] plot[smooth,samples=500] (\x,{-2*(\x)^2 + 11});
	      \draw [dashed] (-2,-\size) -- (-2, \size);
	      \draw [dashed] (2,-\size) -- (2, \size);
	      \draw [color=red,very thick] (-2,0) -- (2,0);
	      \end{scope}

	      \node at ({sqrt(11/2)},0) {$\bullet$};
	      \node at ({sqrt(11/2)},0) [above right] {$(\sqrt{\frac{11}{2}},0)$};

	      \node at (-{sqrt(11/2)},0) {$\bullet$};
	      \node at (-{sqrt(11/2)},0) [above left] {$(-\sqrt{\frac{11}{2}},0)$};;

	      \node at (0,11) {$\bullet$};
	      \node at (0,11) [above right] {$(0,11)$};
	      \end{tikzpicture}
	    </latex-image>
	  </image>
	</figure>
	<p>
	  When <m>x \in (-\infty, -2) \cup (2, \infty)</m>, we obtain the polynomial inequality
	  <md>
	    <mrow>\frac{-2x^2 + 11}{x^2 - 4} \leq 0 \amp\amp \text{Multiply both sides by}\ x^2 - 4</mrow>
	    <mrow>-2x^2 + 11 \leq 0</mrow>
	  </md>
	  Again, as the quadratic <m>y = -2x^2 + 11</m> is a downward facing parabola with roots at <m>\pm \sqrt{11/2}</m>, the solutions to this inequality are on the left- and right-hand sides of the roots
	  <me>\left(-\infty, \cup -\sqrt{\frac{11}{2}}\right] \cup \left[\sqrt{\frac{11}{2}}, \infty\right)</me>
	</p>
	<figure xml:id="fig-rational_example_case_2">
	  <caption>Solutions to the inequality <m>-2x^2 + 11 \leq 0</m></caption>
	  <image xml:id="img-rational_example_case_2">
	    <latex-image xml:id="tikz-rational_example_case_2">
	      \begin{tikzpicture}[scale=0.5]
	      \def\size{12}
	      
	      \path [draw, help lines, opacity=.5]  (-\size,-\size) grid (\size,\size);
	      
	      \draw [very thick,->] (-\size,0) -- (\size+.1,0) node [anchor=south] {$x$};
	      \draw [very thick,->] (0,-\size) -- (0,\size+.1) node [anchor=west] {$y$};
	      
	      \begin{scope}[domain=-5:5]
	      \clip (-\size,-\size) rectangle (\size,\size);
	      \draw [color=blue,thick] plot[smooth,samples=500] (\x,{-2*(\x)^2 + 11});
	      \draw [color=red,very thick] (-\size,0) -- (-{sqrt(11/2)},0);
	      \draw [color=red,very thick] ({sqrt(11/2)},0) -- (\size,0);
	      \end{scope}

	      \node at ({sqrt(11/2)},0) {$\bullet$};
	      \node at ({sqrt(11/2)},0) [above right] {$(\sqrt{\frac{11}{2}},0)$};

	      \node at (-{sqrt(11/2)},0) {$\bullet$};
	      \node at (-{sqrt(11/2)},0) [above left] {$(-\sqrt{\frac{11}{2}},0)$};;

	      \node at (0,11) {$\bullet$};
	      \node at (0,11) [above right] {$(0,11)$};
	      \end{tikzpicture}
	    </latex-image>
	  </image>
	</figure>
	<p>
	  Combining the solutions to each part, we obtain the solution to the rational inequality
	  <me>\left(-\infty, -\sqrt{\frac{11}{2}}\right] \cup (-2, 2) \cup \left[\sqrt{\frac{11}{2}},\infty\right)</me>
	</p>
      </solution>
    </example>

    <worksheet component="notes">
      <title/>
      <page>
	<example>
	  <statement>
	    <p>
	      Solve the equation
	      <me>\frac{x^2 - 1}{x^2 - 4} = 3</me>
	    </p>
	  </statement>
	</example>
      </page>
      <page>
	<example>
	  <statement>
	    <p>
	      Solve the rational inequality
	      <me>\frac{x^2 - 1}{x^2 - 4} \leq 3</me>
	    </p>
	  </statement>
	</example>
      </page>
    </worksheet>
  </subsection>

  <xi:include href="./worksheets/wksht-rational_functions.ptx"/>

  <exercises component="web">
    <introduction>
      <p>
	Solve the following rational inequalities.
      </p>
    </introduction>

    <exercise>
      <statement>
	<p>
	  <m>\dfrac{2x - 1}{3} > 5</m>
	</p>
      </statement>
    </exercise>

    <exercise>
      <statement>
	<p>
	  <m>\dfrac{x^2 - 4}{x + 2} \leq 0</m>
	</p>
      </statement>
    </exercise>

    <exercise>
      <statement>
	<p>
	  <m>\dfrac{3x - 2}{x + 1} \lt 4</m>
	</p>
      </statement>
    </exercise>

    <exercise>
      <statement>
	<p>
	  <m>\dfrac{2x + 1}{x - 3} \geq \dfrac{x + 4}{2}</m>
	</p>
      </statement>
    </exercise>

    <exercise>
      <statement>
	<p>
	  <m>\dfrac{x - 1}{x^2 + 3x + 2} \lt 0</m>
	</p>
      </statement>
    </exercise>

    <exercise>
      <statement>
	<p>
	  <m>\dfrac{2x^2 - 5x + 3}{x^2 - x - 6} \geq \dfrac{x + 2}{x^2 - 4}</m>
	</p>
      </statement>
    </exercise>
  </exercises>
</section>
