<?xml version="1.0" encoding="UTF-8"?>

<section xml:id="sec-sytems_of_planes" xmlns:xi="http://www.w3.org/2001/XInclude">
  <title>Three Dimensions</title>

  <introduction>
    <p>
      When we increase the number of variables in a linear system, we increase the dimension of the ambient space.
      For linear equations with two variables, <m>x</m> and <m>y</m>, we work in the Cartesian plane.
      Linear equations with three variables, <m>x</m>, <m>y</m>, and <m>z</m>, require us to work in three dimensional space
      <me>\R^3 = \left\{(x,y,z) \;\middle\vert\; x,y,z \in \R\right\}.</me>
      This adds additional complexity to the geometric interpretation of solutions to linear equations and systems.
      In particular, a linear equation in three variables no longer represents a line, but rather a <term>plane</term> <mdash/> a figure in space that looks like the Cartesian plane.
      Since this is <em>not</em> a course on linear algebra or multivariable calculus <mdash/> two courses dedicated to the study of higher dimensional spaces <mdash/> we will leave our discussion of the geometry at that, and focus on solving systems algebraically.
    </p>
  </introduction>

  <subsection>
    <title>Systems of Linear Equations in Three Variables</title>
    <p>
      The same terminology and intuition from linear systems in two variables apply to systems of linear equations in three variables.
      First, we start with an adaptation of solutions to equations in two varibles to three variables.
    </p>

    <definition xml:id="def-solution_3d">
      <title>Solution to an Equation in Three Variables</title>
      <statement>
	<p>
	  A <term>solution</term>
	  <idx>
	    <h>Equation</h>
	    <h>Solution</h>
	    <h>Three Variables</h>
	  </idx>
	  to an equation in the variables <m>x</m>, <m>y</m>, and <m>z</m> is an ordered pair <m>(a,b,c)</m> that make the equation true when
	  <ol>
	    <li>
	      <p>
		the first coordinate, <m>a</m>, is substituted into the equation for <m>x</m>,
	      </p>
	    </li>
	    <li>
	      <p>
		the second coordinate, <m>b</m>, is substituted into the equation for <m>y</m>, and
	      </p>
	    </li>
	    <li>
	      <p>
		the third coordinate, <m>c</m>, is substituted into the equation for <m>z</m>.
	      </p>
	    </li>
	  </ol>
	</p>
      </statement>
    </definition>

    <p>
      Next, we generalize the notion of a linear equation from two variables to three.
    </p>

    <definition xml:id="def-linear_equation_3d">
      <title>Standard Form a Linear Equation in Three Variables</title>
      <statement>
	<p>
          The <term>standard form a linear equation</term>
          <idx>
	    <h>Equation</h>
	    <h>Line</h>
	    <h>Standard (Three Variables)</h>
          </idx>
          in the variables <m>x</m>, <m>y</m>, and <m>z</m> is
          <me>ax + by + cz = d,</me>
	  where <m>a</m>, <m>b</m>, and <m>c</m> are not all zero.
	</p>
      </statement>
    </definition>

    <p>
      Now, the notion of a linear system in three variables generalizes naturally.
    </p>
    
    <definition xml:id="def-system_planes">
      <statement>
	<p>
	  A <term>system of <m>m</m> linear equations in the variables <m>x</m>, <m>y</m>, and <m>z</m></term>
	  <idx>
	    <h>Linear System</h>
	    <h>Three Variables</h>
	  </idx>
	  is a collection of <m>m</m> equations
	  <me>
	    \begin{array}{ccccccc}
	    a_1x \amp + \amp b_1y \amp + \amp c_1z \amp=\amp d_1\\
	    a_2x \amp + \amp b_2y \amp + \amp c_2z \amp=\amp d_2\\
	    \vdots \amp \amp \vdots \amp \amp \vdots \amp \amp\vdots\\
	    a_mx \amp + \amp b_my \amp + \amp c_3z \amp=\amp d_m
	    \end{array}
	  </me>
	</p>
	<p>
	  A <term>solution</term>
	  <idx>
	    <h>Linear System</h>
	    <h>Three Variables</h>
	    <h>Solution</h>
	  </idx>
	  to the system is a point <m>(a,b,c)</m> that is a <xref ref="def-solution_3d" text="custom">solution</xref> for <em>every</em> equation in the system.
	</p>
      </statement>
    </definition>
  </subsection>
  
  <subsection>
    <title>Solving Linear Systems with Three Equations</title>
    <p>
      Fortunately, the method of substitution also generalizes naturally.
      To solve a system of equations in three variables, solve one equation of your choosing for one of the variables and substitute into the other equations.
      This reduces to a linear system in two equations, which we already know how to solve.
    </p>

    <example component="web">
      <statement>
	<p>
	  Solve the system
	  <md>
	    <mrow>2x + z \amp = 5</mrow>
	    <mrow>2x + y + z \amp = 7</mrow>
	    <mrow>x + z \amp = 4</mrow>
	  </md>
	</p>
      </statement>
      <solution>
	<p>
	  We choose to solve the last equation for <m>z</m> in terms of <m>x</m>:
	  <me>z = 4 - x.</me>
	  Substitute <m>4 - x</m> for <m>z</m> in the other two equations to reduce to a system of two linear equations in the variables <m>x</m> and <m>y</m>,
	  <md>
	    <mrow>2x + (4 - x) = x + 4\amp = 5</mrow>
	    <mrow>2x + y + (4 - x) = x + y + 4\amp = 7</mrow>
	  </md>
	  Subtract <m>4</m> from both sides of the equation <m>x + 4 = 5</m>:
	  <me>x = 5 - 4 = 1.</me>
	  Substitute <m>x = 1</m> into the equation <m>x + y + 4 = 7</m> to solve for <m>y</m>:
	  <md>
	    <mrow>\amp x + y + 4 = 7 \amp\amp \text{Substitute}\ 1\ \text{for}\ x</mrow>
	    <mrow>\amp 1 + y + 4 = y + 5 = 7 \amp\amp \text{Subtract}\ 5\ \text{from both sides}</mrow>
	    <mrow>\amp y = 2.</mrow>
	  </md>
	  Finally, substitute <m>x = 1</m> into the equation for <m>z</m> to find
	  <me>z = 4 - x = 4 - 1 = 3.</me>
	  Therefore there is exactly one solution to the system, <m>(1,2,3)</m>.
	</p>
      </solution>
    </example>

    <p component="web">
      Unlike linear systems with two equations, it is possible for to obtain a dependent system even when the equations are not the same.
    </p>

    <example component="web">
      <statement>
	<p>
	  Solve the system
	  <md>
	    <mrow>x + y + z \amp= 1</mrow>
	    <mrow>x + y + 2z \amp= 2</mrow>
	  </md>
	</p>
      </statement>
      <solution>
	<p>
	  Solve the first equation for <m>z</m> in terms of <m>x</m> and <m>y</m>:
	  <me>z = 1 - x - y.</me>
	  Substitute for <m>z</m> in the second equation to obtain
	  <me>2 = x + y + 2(1 - x - y) = x + y + 2 - 2x - 2y = -x - y + 2</me>
	  and solve for <m>y</m> in terms of <m>x</m>
	  <md>
	    <mrow>\amp 2 = -x - y + 2 \amp\amp \text{Add}\ y\ \text{to both sides}</mrow>
	    <mrow>\amp y + 2 = -x + 2 \amp\amp \text{Subtract}\ 2\ \text{from both sides}</mrow>
	    <mrow>\amp y = -x.</mrow>
	  </md>
	  Finally, substitute <m>y = -x</m> into the equation <m>z = 1 - x - y</m> to obtain
	  <me>z = 1 - x - (-x) = 1 - x + x = 1.</me>
	  Therefore the solutions to this system form the line in <m>\R^3</m>
	  <me>\left\{(x, -x, 1) \;\middle\vert\; x \in \R\right\}.</me>
	</p>
      </solution>
    </example>

    <worksheet component="notes">
      <title/>
      <page>
	<example>
	  <statement>
	    <p>
	      Solve the system
	      <md>
		<mrow>2x + z \amp = 5</mrow>
		<mrow>2x + y + z \amp = 7</mrow>
		<mrow>x + z \amp = 4</mrow>
	      </md>
	    </p>
	  </statement>
	</example>
      </page>

      <page>
	<p>
	  Unlike linear systems with two equations, it is possible for to obtain a dependent system even when the equations are not the same.
	  <example>
	    <statement>
	      <p>
		Solve the system
		<md>
		  <mrow>x + y + z \amp= 1</mrow>
		  <mrow>x + y + 2z \amp= 2</mrow>
		</md>
	      </p>
	    </statement>
	  </example>
	</p>
      </page>
    </worksheet>
  </subsection>
</section>
