<?xml version="1.0" encoding="UTF-8"?>

<section xml:id="sec-linear_functions" xmlns:xi="http://www.w3.org/2001/XInclude">
  <title>Linear Functions</title>
  
  <introduction>
    <p>
      In this section, we study a special kind of polynomial known as a <em>linear function</em>.
      As we will see, the name linear comes from the fact that the graph of such a function is always a line.
    </p>
  </introduction>

  <subsection>
    <title>Linear Functions and Slope</title>
    <definition xml:id="def-linear_function">
      <title>Linear Function</title>
      <statement>
	<p>
	  A function <m>f \colon \R \to \R</m> is <term>linear</term>
	  <idx>
	    <h>Function</h>
	    <h>Linear</h>
	  </idx>
	  if the <xref ref="def-average_rate_of_change" text="title"/> of <m>f</m> is constant.
	  That is, there exists a number <m>m</m> such that for all numbers <m>a</m> and <m>b</m>
	  <me>m = \frac{f(b) - f(a)}{b - a}.</me>
	  We call the number <m>m</m> the <term>slope</term>
	  <idx>
	    <h>Function</h>
	    <h>Linear</h>
	    <h>Slope</h>
	  </idx>
	  of <m>f</m>.
	  The number <m>b</m> is the <m>y</m>-coordinate of the <xref ref="def-y_intercept" text="title"/> <m>\left(0, b\right)</m>.
	</p>
      </statement>
    </definition>

    <p>
      In order to find the equation of a linear function, it is enough to know the slope, <m>m</m>, and the value of the function for a single <m>x</m>-value.
      The simplest point to find is the <xref ref="def-y_intercept" text="title"/>: the <m>x</m>-coordinate is <m>0</m> and the <m>y</m>-coordinate is <m>b = f(0)</m>.
      If we write <m>y = f(x)</m>, then by <xref ref="def-linear_function"/>
      <me>m = \frac{f(x) - f(0)}{x - 0} = \frac{y - b}{x}.</me>
      We obtain the equation for the function by solving the equation for <m>y</m> in terms of <m>x</m>
      <md>
	<mrow>m \amp= \frac{y - b}{x} \amp\amp \text{Multiply both sides by}\ x</mrow>
	<mrow>mx \amp = y - b \amp\amp \text{Add}\ b\ \text{to both sides}</mrow>
	<mrow>mx + b \amp = y \amp\amp \text{Swap sides}</mrow>
	<mrow>y \amp = mx + b \amp\amp \text{Replace}\ y\ \text{with}\ f(x)</mrow>
	<mrow>f(x) \amp = mx + b</mrow>
      </md>
    </p>

    <theorem xml:id="thm-slope_intercept">
      <title>The Slope-Intercept Form of a Line</title>
      <p>
	The <term>slope-intercept form of a linear function</term>
	<idx>
	  <h>Function</h>
	  <h>Linear</h>
	  <h>Slope-Intercept Form</h>
	</idx>
	is
	<me>f(x) = mx + b
	\quad\text{or}\quad
	y = mx + b,</me>
	where <m>m</m> is the slope or average rate of change of <m>f</m>.
      </p>
    </theorem>
  </subsection>
  
  <subsection>
    <title>Graphing Linear Functions</title>
    <p>
      Consider a linear function <m>y = mx + b</m> with <m>m \neq 0</m>.
      Recall that the <xref ref="def-graph" text="title"/> of an equation consists of all points <m>(x,y)</m> that are a <xref ref="def-solution" text="title"/> to the equation.
      The graph of a linear equation is always a line.
      We can graph the equation by finding any two points on the line and drawing a line through them.
      In general, the two points that are simplest to find are the two intercepts.
    </p>
    

    <p>
      We find the <xref ref="def-x_intercept" text="title"/> by substituting <m>0</m> for <m>y</m> and solving the resulting equation for <m>x</m>
      <md>
	<mrow>0 \amp= mx + b \amp\amp \text{Subtract}\ b\ \text{from both sides}</mrow>
	<mrow>mx \amp= -b \amp\amp \text{Divide both sides by}\ m</mrow>
	<mrow>x \amp = -\frac{b}{m}.</mrow>
      </md>
    </p>
    
    <theorem xml:id="thm-linear_x_intercept">
      <statement>
	<p>
	  The <xref ref="def-x_intercept" text="title"/> of the linear function <m>y = mx + b</m> with <m>m \neq 0</m> is the point
	  <me>\left(-\frac{b}{m}, 0\right).</me>
	</p>
      </statement>
    </theorem>

    <example xml:id="example-x_intercept_2x_3y_6">
      <statement>
	<p>
	  Find the <m>x</m>-intercept of the linear equation <m>y = -\frac{2}{3}x + 2</m>.
	</p>
      </statement>
      <solution>
	<p>
	  To find the <m>x</m>-intercept of the linear equation <m>y = -\frac{2}{3}x + 2</m>, we substitute <m>0</m> for <m>y</m> to get
	  <md>
	    <mrow>0 \amp= -\frac{2}{3}x + 2 \amp\amp \text{Add}\ -\frac{2}{3}x\ \text{to both sides}</mrow>
	    <mrow>\frac{2}{3}x \amp = 2 \amp\amp \text{Multiply both sides by}\ \frac{3}{2}</mrow>
	    <mrow>x \amp = \left(\frac{3}{2}\right) \amp\amp \text{Simplify}</mrow>
	    <mrow>x \amp = 3.</mrow>
	  </md>
	  Therefore the <m>x</m>-intercept of the linear equation <m>y = -\frac{2}{3}x + 2</m> is the point <m>(3,0)</m>.
	</p>
      </solution>
    </example>
    
    <p>
      We find the <xref ref="def-y_intercept" text="title"/> by substituting <m>0</m> for <m>x</m> and solving the resulting equation for <m>y</m>
      <md>
	<mrow>y \amp = m(0) + b \amp\amp \text{Simplify}</mrow>
	<mrow>y \amp = b.</mrow>
      </md>
    </p>
    
    <example>
      <statement>
	<p>Graph the equation <m>y = -\frac{2}{3}x + 2</m>.</p>
      </statement>
      <solution>
	<p>
	  In <xref ref="example-x_intercept_2x_3y_6"/> we found that <m>(3,0)</m> is the <m>x</m>-intercept for the function <m>y = -\frac{2}{3}x + 2</m>.
	  The <xref ref="def-y_intercept" text="title"/> for the function <m>y = -\frac{2}{3}x + 2</m> is the point <m>(0, 2)</m>.
	  To graph the equation <m>y = -\frac{2}{3}x + 2</m>, we simply need to plot these two points and draw a straight line through them.
	</p>
	<figure xml:id="fig-2x_3y_6">
	  <caption>The graph of <m>y = -\frac{2}{3}x + 2</m>.</caption>
	  <image xml:id="img-2x_3y_6">
	    <latex-image >
	      <xi:include parse="text" href="tex/2x_3y_6.tex"/>
	    </latex-image>
	  </image>
	</figure>	
      </solution>
    </example>
  </subsection>

  <xi:include href="worksheets/wksht-working_with_linear_equations.ptx"/>
</section>
